src/Framework/KnownAnnotate.v
@@ -10,198 +10,1054 @@ From Framework Require Import Util ANF0 ANF Annotate Erase.
 Module A0 := ANF0.
 Module A1 := ANF.
 
-(* Known Function Analysis With A Single Exposed Web Id *)
+Module M <: Annotate.
 
-(* Outline: *)
-(* 1. run `analyze` to build `K : known_map` for every function identifiers (assume unique names) in the program with nonexposed web ids (Note it is not necessary to require them to be distinct though) *)
-(* 2. follow `escape_fun_exp` as in CertiCoq to filter `K` so that its domain satisfies `known_fun` *)
-(* 3. rewrite based on `K` *)
+  (* Known Function Analysis With A Single Exposed Web Id *)
 
-(* Step 3 is the main step we are establishing here *)
+  (* Outline: *)
+  (* 1. run `analyze` to build `K : known_map` for every function identifiers (assume unique names) in the program with nonexposed web ids (Note it is not necessary to require them to be distinct though) *)
+  (* 2. follow `escape_fun_exp` as in CertiCoq to filter `K` so that its domain satisfies `known_fun` *)
+  (* 3. rewrite based on `K` *)
 
-Definition known_map := M.t web.
+  (* Step 3 is the main step we are establishing here *)
 
-Parameter analyze : A0.exp -> known_map.
+  Definition known_map := M.t web.
 
-(* Specification for the *result* of `analyze`, or `K` *)
-(* Similar to CertiCoq's `Known_exp` *)
-Inductive known_fun (S : Ensemble var) : A0.exp -> Prop :=
-| Known_Ret :
-  forall x,
-    (~ x \in S) ->
-    known_fun S (A0.Eret x)
+  Parameter analyze : A0.exp -> known_map.
 
-| Known_App :
-  forall f ys,
-    (f \in S) ->
-    Disjoint _ (FromList ys) S ->
-    known_fun S (A0.Eapp f ys)
-
-| Known_LetApp :
-  forall x f ys e,
-    (f \in S) ->
-    (~ x \in S) -> (* intermediate result shouldn't be known fun *)
-    Disjoint _ (FromList ys) S ->
-    known_fun S e ->
-    known_fun S (A0.Eletapp x f ys e)
-
-| Known_Fun:
-  forall f xs e k,
-    (f \in S) ->
-    Disjoint _ (FromList xs) S ->
-    known_fun S e ->
-    known_fun S k ->
-    known_fun S (A0.Efun f xs e k)
-
-| Known_Constr :
-  forall x ys ct e,
-    (~ x \in S) -> (* constructors are not known functions, but they can still be known exp *)
-    Disjoint _ (FromList ys) S ->
-    known_fun S e ->
-    known_fun S (A0.Econstr x ct ys e)
-
-| Known_Proj :
-  forall x n y e,
-    (~ x \in S) ->
-    (~ y \in S) ->
-    known_fun S e ->
-    known_fun S (A0.Eproj x n y e)
-
-| Known_Case_nil:
-  forall x,
-    (~ x \in S) ->
-    known_fun S (A0.Ecase x [])
-
-| Known_Case_hd:
-  forall x c e ce,
-    (~ x \in S) ->
-    known_fun S e ->
-    known_fun S (A0.Ecase x ce) ->
-    known_fun S (A0.Ecase x ((c, e) :: ce)).
-
-Hint Constructors known_fun : core.
-
-Definition known_map_inv K :=
-  forall f w,
-    K ! f = Some w ->
-    ~ (w \in Exposed).
-
-Definition analyze_spec K e :=
-  known_fun (Dom_map K) e /\
-  known_map_inv K.
-
-Axiom analyze_sound :
-  forall (e : A0.exp),
-    analyze_spec (analyze e) e.
-
-(*
-Definition known_map_bound (K : known_map) e :=
-  (Dom_map K) \subset (A0.bound_var e).
-
-Definition known_map_exclude (K : known_map) Γ :=
-  Disjoint _ (Dom_map K) Γ.
-
-Parameter join : known_map -> known_map -> known_map.
-
-Definition join_spec (K1 K2 K3 : known_map) :=
-  forall x,
-    (forall w, K1 ! x = Some w -> K2 ! x = None -> K3 ! x = Some w) /\
-    (forall w, K1 ! x = None -> K2 ! x = Some w -> K3 ! x = Some w) /\
-    (K1 ! x = None -> K2 ! x = None -> K3 ! x = None).
-
-Axiom join_sound :
-  forall K1 K2,
-    Disjoint _ (Dom_map K1) (Dom_map K2) ->
-    join_spec K1 K2 (join K1 K2).
-
-Lemma Disjoint_join_known_map_inv K1 K2 :
-  Disjoint _ (Dom_map K1) (Dom_map K2) ->
-  known_map_inv K1 ->
-  known_map_inv K2 ->
-  known_map_inv (join K1 K2).
-Proof.
-  intros HD HK1 HK2.
-  pose proof (join_sound _ _ HD) as HJ.
-  unfold join_spec, known_map_inv in *.
-  intros.
-  intros Hc.
-  destruct (HJ f) as [Hf1 [Hf2 Hf3]].
-  clear HJ.
-  destruct (K1 ! f) eqn:HK1f;
-    destruct (K2 ! f) eqn:HK2f;
-    remember (join K1 K2) as K3.
-  - inv HD.
-    apply (H0 f).
-    constructor; unfold Ensembles.In, Dom_map; eauto.
-  - assert (K3 ! f = Some w0) by (eapply Hf1; eauto).
-    rewrite H in H0; inv H0.
-    eapply HK1; eauto.
-  - assert (K3 ! f = Some w0) by (eapply Hf2; eauto).
-    rewrite H in H0; inv H0.
-    eapply HK2; eauto.
-  - assert (K3 ! f = None) by (eapply Hf3; eauto).
-    rewrite H in H0; inv H0.
-Qed.
- *)
-
-Parameter w0 : web.
-Axiom w0_exposed : w0 \in Exposed.
-Axiom Exposed_singleton : forall w, w \in Exposed -> w = w0.
-
-Theorem Exposed_nonempty : exists w, w \in Exposed.
-Proof. exists w0. apply w0_exposed. Qed.
-
-Section Known.
-  Variable K : known_map.
-
-  (* Specification based on `known_fun` but incorporate unknown cases *)
-  Inductive trans_ (Γ : A0.vars) : A0.exp -> A1.exp -> Prop :=
-  | Trans_ret :
+  (* Specification for the *result* of `analyze`, or `K` *)
+  (* Similar to CertiCoq's `Known_exp` *)
+  Inductive known_fun (S : Ensemble var) : A0.exp -> Prop :=
+  | Known_Ret :
     forall x,
-      K ! x = None ->
+      (~ x \in S) ->
+      known_fun S (A0.Eret x)
+
+  | Known_App :
+    forall f ys,
+      (f \in S) ->
+      Disjoint _ (FromList ys) S ->
+      known_fun S (A0.Eapp f ys)
+
+  | Known_LetApp :
+    forall x f ys e,
+      (f \in S) ->
+      (~ x \in S) -> (* intermediate result shouldn't be known fun *)
+      Disjoint _ (FromList ys) S ->
+      known_fun S e ->
+      known_fun S (A0.Eletapp x f ys e)
+
+  | Known_Fun:
+    forall f xs e k,
+      (f \in S) ->
+      Disjoint _ (FromList xs) S ->
+      known_fun S e ->
+      known_fun S k ->
+      known_fun S (A0.Efun f xs e k)
+
+  | Known_Constr :
+    forall x ys ct e,
+      (~ x \in S) -> (* constructors are not known functions, but they can still be known exp *)
+      Disjoint _ (FromList ys) S ->
+      known_fun S e ->
+      known_fun S (A0.Econstr x ct ys e)
+
+  | Known_Proj :
+    forall x n y e,
+      (~ x \in S) ->
+      (~ y \in S) ->
+      known_fun S e ->
+      known_fun S (A0.Eproj x n y e)
+
+  | Known_Case_nil:
+    forall x,
+      (~ x \in S) ->
+      known_fun S (A0.Ecase x [])
+
+  | Known_Case_hd:
+    forall x c e ce,
+      (~ x \in S) ->
+      known_fun S e ->
+      known_fun S (A0.Ecase x ce) ->
+      known_fun S (A0.Ecase x ((c, e) :: ce)).
+
+  Hint Constructors known_fun : core.
+
+  Definition known_map_inv K :=
+    forall f w,
+      K ! f = Some w ->
+      ~ (w \in Exposed).
+
+  Definition web_map := known_map.
+
+  Definition web_map_inv := known_map_inv.
+
+  Definition analysis_spec (K : web_map) e :=
+    known_fun (Dom_map K) e.
+
+  Definition analyze_spec K e :=
+    analysis_spec K e /\
+    known_map_inv K.
+
+  Axiom analyze_sound :
+    forall (e : A0.exp),
+      analyze_spec (analyze e) e.
+
+  Parameter w0 : web.
+  Axiom w0_exposed : w0 \in Exposed.
+  Axiom Exposed_singleton : forall w, w \in Exposed -> w = w0.
+
+  Theorem Exposed_nonempty : exists w, w \in Exposed.
+  Proof. exists w0. apply w0_exposed. Qed.
+
+  Section Known.
+    Variable K : known_map.
+
+    (* Specification based on `known_fun` but incorporate unknown cases *)
+    Inductive trans_ (Γ : A0.vars) : A0.exp -> A1.exp -> Prop :=
+    | Trans_ret :
+      forall x,
+        K ! x = None ->
+        (x \in Γ) ->
+        trans_ Γ (A0.Eret x) (A1.Eret x)
+
+    | Trans_fun_known :
+      forall {f w xs e k e' k'},
+        K ! f = Some w ->
+        (~ w \in Exposed) ->
+        Disjoint _ (FromList xs) (Dom_map K) ->
+
+        trans_ (FromList xs :|: (f |: Γ)) e e' ->
+        trans_ (f |: Γ) k k' ->
+        trans_ Γ (A0.Efun f xs e k) (A1.Efun f w xs e' k')
+
+    | Trans_fun_unknown :
+      forall {f xs e k e' k'},
+        K ! f = None ->
+        Disjoint _ (FromList xs) (Dom_map K) ->
+
+        trans_ (FromList xs :|: (f |: Γ)) e e' ->
+        trans_ (f |: Γ) k k' ->
+        trans_ Γ (A0.Efun f xs e k) (A1.Efun f w0 xs e' k')
+
+    | Trans_app_known :
+      forall {f w xs},
+        K ! f = Some w ->
+        (~ w \in Exposed) ->
+        Disjoint _ (FromList xs) (Dom_map K) ->
+
+        (f \in Γ) ->
+        (FromList xs \subset Γ) ->
+        trans_ Γ (A0.Eapp f xs) (A1.Eapp f w xs)
+
+    | Trans_app_unknown :
+      forall {f xs},
+        K ! f = None ->
+        Disjoint _ (FromList xs) (Dom_map K) ->
+
+        (f \in Γ) ->
+        (FromList xs \subset Γ) ->
+        trans_ Γ (A0.Eapp f xs) (A1.Eapp f w0 xs)
+
+    | Trans_letapp_known :
+      forall {x f w xs k k'},
+        K ! f = Some w ->
+        (~ w \in Exposed) ->
+        Disjoint _ (FromList xs) (Dom_map K) ->
+        K ! x = None ->
+
+        (f \in Γ) ->
+        (FromList xs \subset Γ) ->
+        trans_ (x |: Γ) k k' ->
+        trans_ Γ (A0.Eletapp x f xs k) (A1.Eletapp x f w xs k')
+
+    | Trans_letapp_unknown :
+      forall {x f xs k k'},
+        K ! f = None ->
+        Disjoint _ (FromList xs) (Dom_map K) ->
+        K ! x = None ->
+
+        (f \in Γ) ->
+        (FromList xs \subset Γ) ->
+        trans_ (x |: Γ) k k' ->
+        trans_ Γ (A0.Eletapp x f xs k) (A1.Eletapp x f w0 xs k')
+
+    (* data webs are all exposed *)
+
+    | Trans_constr :
+      forall {x t xs k k'},
+        K ! x = None ->
+        Disjoint _ (FromList xs) (Dom_map K) ->
+
+        (FromList xs \subset Γ) ->
+        trans_ (x |: Γ) k k' ->
+        trans_ Γ (A0.Econstr x t xs k) (A1.Econstr x w0 t xs k')
+
+    | Trans_proj :
+      forall {x y k k' n},
+        K ! x = None ->
+        K ! y = None ->
+
+        (y \in Γ) ->
+        trans_ (x |: Γ) k k' ->
+        trans_ Γ (A0.Eproj x n y k) (A1.Eproj x w0 n y k')
+
+    | Trans_case_nil :
+      forall {x},
+        K ! x = None ->
+        (x \in Γ) ->
+        trans_ Γ (A0.Ecase x []) (A1.Ecase x w0 [])
+
+    | Trans_case_cons :
+      forall {x e e' t cl cl'},
+        K ! x = None ->
+        (x \in Γ) ->
+        trans_ Γ e e' ->
+        trans_ Γ (A0.Ecase x cl) (A1.Ecase x w0 cl') ->
+        trans_ Γ (A0.Ecase x ((t, e) :: cl)) (A1.Ecase x w0 ((t, e') :: cl')).
+
+    Hint Constructors trans_ : core.
+
+    Definition trans := trans_.
+
+    Hint Unfold trans : core.
+
+    Lemma known_fun_trans e :
+      known_map_inv K ->
+      known_fun (Dom_map K) e ->
+      forall Γ,
+        (A0.occurs_free e) \subset Γ ->
+        exists e', trans Γ e e'.
+    Proof.
+      unfold known_map_inv.
+      intros HK H.
+      induction H; simpl; intros.
+      - exists (A1.Eret x); auto.
+      - apply Dom_map_eq in H.
+        destruct H as [w Hw].
+        exists (A1.Eapp f w ys); econstructor; eauto.
+        eapply A0.free_app_xs_inv; eauto.
+      - apply Dom_map_eq in H.
+        destruct H as [w Hw].
+        destruct (IHknown_fun (x |: Γ)) as [e' He']; auto.
+        eapply A0.free_letapp_k_inv; eauto.
+        exists (A1.Eletapp x f w ys e'); econstructor; eauto.
+        eapply A0.free_letapp_xs_inv; eauto.
+      - apply Dom_map_eq in H.
+        destruct H as [w Hw].
+        destruct (IHknown_fun1 (FromList xs :|: (f |: Γ))) as [e' He']; auto.
+        eapply A0.free_fun_e_inv; eauto.
+        destruct (IHknown_fun2 (f |: Γ)) as [k' Hk']; auto.
+        eapply A0.free_fun_k_inv; eauto.
+        exists (A1.Efun f w xs e' k'); econstructor; eauto.
+      - destruct (IHknown_fun (x |: Γ)) as [e' He']; auto.
+        eapply A0.free_constr_k_inv; eauto.
+        exists (A1.Econstr x w0 ct ys e'); econstructor; eauto.
+        eapply A0.free_constr_xs_inv; eauto.
+      - destruct (IHknown_fun (x |: Γ)) as [e' He']; auto.
+        eapply A0.free_proj_k_inv; eauto.
+        exists (A1.Eproj x w0 n y e'); econstructor; eauto.
+      - exists (A1.Ecase x w0 []); econstructor; eauto.
+      - destruct (IHknown_fun1 Γ) as [e' He']; auto.
+        eapply A0.free_case_hd_inv; eauto.
+        destruct (IHknown_fun2 Γ) as [c' Hc']; auto.
+        eapply A0.free_case_tl_inv; eauto.
+        inv Hc'.
+        + exists (A1.Ecase x w0 [(c, e')]); econstructor; eauto.
+        + exists (A1.Ecase x w0 ((c, e') :: (t, e'0) :: cl')); econstructor; eauto.
+    Qed.
+
+    Theorem trans_total e :
+      web_map_inv K ->
+      analysis_spec K e ->
+      exists e', trans (A0.occurs_free e) e e'.
+    Proof.
+      intros.
+      eapply known_fun_trans; eauto.
+      apply Included_refl.
+    Qed.
+
+    Lemma trans_exp_inv {Γ e e'} :
+      trans Γ e e' ->
+      (A1.occurs_free e') \subset (A0.occurs_free e).
+    Proof.
+      unfold Ensembles.Included, Ensembles.In.
+      intros H.
+      induction H; simpl; intros; auto.
+      - inv H1; auto.
+      - inv H4; auto.
+      - inv H3; auto.
+      - inv H4; auto.
+      - inv H3; auto.
+      - inv H6; auto.
+      - inv H5; auto.
+      - inv H3; auto.
+      - inv H3; auto.
+      - inv H1; auto.
+      - inv H3; auto.
+    Qed.
+
+    Theorem trans_erase e1 e2 e1' :
+      trans (A0.occurs_free e1) e1 e1' ->
+      Erase.trans (A1.occurs_free e1') e1' e2 ->
+      e1 = e2.
+    Proof.
+      unfold trans.
+      intro H.
+      revert e2.
+      induction H; simpl; intros.
+      - inv H1; auto.
+      - inv H4; auto.
+        erewrite IHtrans_1 with (e2 := e'0); eauto.
+        + erewrite IHtrans_2 with (e2 := k'0); eauto.
+          eapply Erase.trans_exp_strengthen; eauto.
+          eapply A1.free_fun_k_subset; eauto.
+        + eapply Erase.trans_exp_strengthen; eauto.
+          eapply A1.free_fun_e_subset; eauto.
+      - inv H3; auto.
+        erewrite IHtrans_1 with (e2 := e'0); eauto.
+        + erewrite IHtrans_2 with (e2 := k'0); eauto.
+          eapply Erase.trans_exp_strengthen; eauto.
+          eapply A1.free_fun_k_subset; eauto.
+        + eapply Erase.trans_exp_strengthen; eauto.
+          eapply A1.free_fun_e_subset; eauto.
+      - inv H4; auto.
+      - inv H3; auto.
+      - inv H6; auto.
+        erewrite IHtrans_ with (e2 := k'0); eauto.
+        eapply Erase.trans_exp_strengthen; eauto.
+        eapply A1.free_letapp_k_subset; eauto.
+      - inv H5; auto.
+        erewrite IHtrans_ with (e2 := k'0); eauto.
+        eapply Erase.trans_exp_strengthen; eauto.
+        eapply A1.free_letapp_k_subset; eauto.
+      - inv H3; auto.
+        erewrite IHtrans_ with (e2 := k'0); eauto.
+        eapply Erase.trans_exp_strengthen; eauto.
+        eapply A1.free_constr_k_subset; eauto.
+      - inv H3; auto.
+        erewrite IHtrans_ with (e2 := k'0); eauto.
+        eapply Erase.trans_exp_strengthen; eauto.
+        eapply A1.free_proj_k_subset; eauto.
+      - inv H1; auto.
+      - inv H3; auto.
+        erewrite IHtrans_1 with (e2 := e'0); eauto.
+        assert (A0.Ecase x cl = A0.Ecase x cl'0).
+        {
+          erewrite IHtrans_2 with (e2 := (A0.Ecase x cl'0)); eauto.
+          eapply Erase.trans_exp_strengthen; eauto.
+          eapply A1.free_case_tl_subset; eauto.
+        }
+        inv H3; auto.
+        eapply Erase.trans_exp_strengthen; eauto.
+        eapply A1.free_case_hd_subset; eauto.
+    Qed.
+
+    (* Cross-language Logical Relations *)
+    (* Note these are parameterized by the known_map, `K` *)
+    Definition R' (P : nat -> A0.val -> A1.wval -> Prop) (i : nat) (r1 : A0.res) (r2 : A1.res) :=
+      match r1, r2 with
+      | A0.OOT, A1.OOT => True
+      | A0.Res v1, A1.Res v2 => P i v1 v2
+      | _, _ => False
+      end.
+
+    Definition E' (P : nat -> A0.val -> A1.wval -> Prop) (ex : bool) (i : nat) (ρ1 : A0.env) (e1 :A0.exp) (ρ2 : A1.env) (e2 : A1.exp) : Prop :=
+      forall j1 r1,
+        j1 <= i ->
+        A0.bstep_fuel ρ1 e1 j1 r1 ->
+        exists j2 r2,
+          A1.bstep_fuel ex ρ2 e2 j2 r2 /\
+          R' P (i - j1) r1 r2.
+
+    Fixpoint V (i : nat) (v1 : A0.val) (wv2 : A1.wval) {struct i} : Prop :=
+      wf_val wv2 /\
+      match wv2 with
+      | A1.TAG _ w2 v2 =>
+          match v1, v2 with
+          | A0.Vconstr c1 vs1, A1.Vconstr c2 vs2 =>
+              exposed wv2 /\
+              c1 = c2 /\
+              match i with
+              | 0 => length vs1 = length vs2
+              | S i0 => Forall2 (V i0) vs1 vs2
+              end
+
+          | A0.Vfun f1 ρ1 xs1 e1, A1.Vfun f2 ρ2 xs2 e2 =>
+              (* note function arguments and result are always exposed regardless of whether a function is known or unknown *)
+              f1 = f2 /\
+              length xs1 = length xs2 /\
+              match K ! f1 with
+              | None => (* unknown *)
+                  exposed wv2 /\
+                  match i with
+                  | 0 => True
+                  | S i0 =>
+                      forall j vs1 vs2 ρ3 ρ4,
+                        j <= i0 ->
+                        Forall exposed vs2 ->
+                        Forall2 (V (i0 - (i0 - j))) vs1 vs2 ->
+                        set_lists xs1 vs1 (M.set f1 (A0.Vfun f1 ρ1 xs1 e1) ρ1) = Some ρ3 ->
+                        set_lists xs2 vs2 (M.set f2 (Tag w2 (A1.Vfun f2 ρ2 xs2 e2)) ρ2) = Some ρ4 ->
+                        E' V true (i0 - (i0 - j)) ρ3 e1 ρ4 e2
+                  end
+
+              | Some w1 => (* known *)
+                  w1 = w2 /\
+                  (~ w1 \in Exposed) /\
+                  match i with
+                  | 0 => True
+                  | S i0 =>
+                      forall j vs1 vs2 ρ3 ρ4,
+                        j <= i0 ->
+                        Forall exposed vs2 ->
+                        Forall2 (V (i0 - (i0 - j))) vs1 vs2 ->
+                        set_lists xs1 vs1 (M.set f1 (A0.Vfun f1 ρ1 xs1 e1) ρ1) = Some ρ3 ->
+                        set_lists xs2 vs2 (M.set f2 (Tag w2 (A1.Vfun f2 ρ2 xs2 e2)) ρ2) = Some ρ4 ->
+                        E' V true (i0 - (i0 - j)) ρ3 e1 ρ4 e2
+                  end
+              end
+          | _, _ => False
+          end
+      end.
+
+    Definition R := (R' V).
+
+    Definition E := (E' V).
+
+    (* Lemmas about [wf_val], [wf_res], and [wf_env] *)
+    Lemma V_wf_val_r {i v1 v2}:
+      V i v1 v2 ->
+      wf_val v2.
+    Proof.
+      intros HV.
+      destruct i; simpl in *;
+        destruct HV as [Hv2 _]; auto.
+    Qed.
+
+    Lemma V_wf_val_Forall_r {i vs1 vs2} :
+      Forall2 (V i) vs1 vs2 ->
+      Forall wf_val vs2.
+    Proof.
+      intros.
+      induction H; auto.
+      constructor; auto.
+      eapply V_wf_val_r; eauto.
+    Qed.
+
+    Lemma V_wf_res_r {i v1 v2}:
+      V i v1 v2 ->
+      wf_res (Res v2).
+    Proof.
+      intros HV.
+      constructor.
+      eapply V_wf_val_r; eauto.
+    Qed.
+
+    Lemma R_wf_res_l {i r1 r2} :
+      R i r1 r2 ->
+      wf_res r2.
+    Proof.
+      unfold R.
+      intros.
+      destruct r1; destruct r2; try contradiction; auto.
+      constructor.
+      eapply V_wf_val_r; eauto.
+    Qed.
+
+    (* Inversion Lemmas *)
+    Lemma R_res_inv_l i v1 r2 :
+      R i (A0.Res v1) r2 ->
+      exists v2, r2 = A1.Res v2 /\ V i v1 v2.
+    Proof.
+      intros.
+      destruct r2; simpl in *; try contradiction.
+      eexists; split; eauto.
+    Qed.
+
+    (* Environment Relation *)
+    Definition same_id x wv2 :=
+      match wv2 with
+      | A1.TAG _ w2 v2 =>
+          match v2 with
+          | A1.Vfun f2 ρ2 xs2 e2 => f2 = x
+          | A1.Vconstr c2 vs2 => True
+          end
+      end.
+
+    Lemma same_id_fun f w f1 t l e:
+      same_id f (TAG val w (Vfun f1 t l e)) -> f1 = f.
+    Proof. unfold same_id; simpl; auto. Qed.
+
+    Definition binding_inv x v :=
+      (forall w, K ! x = Some w -> same_id x v) /\
+        (K ! x = None -> exposed v).
+
+    Lemma binding_inv_exposed x v :
+      (K ! x = None) ->
+      exposed v ->
+      binding_inv x v.
+    Proof.
+      unfold binding_inv.
+      intros.
+      split; intros; auto.
+      rewrite H in H1; discriminate.
+    Qed.
+
+    Lemma binding_inv_exposed_Forall xs :
+      forall vs,
+        Disjoint _ (FromList xs) (Dom_map K) ->
+        length xs = length vs ->
+        Forall exposed vs ->
+        Forall2 binding_inv xs vs.
+    Proof.
+      induction xs; simpl; intros;
+        destruct vs; try discriminate; auto.
+      inv H1.
+      apply Disjoint_FromList_cons_inv in H.
+      inv H.
+      constructor; auto.
+      apply binding_inv_exposed; auto.
+    Qed.
+
+    Lemma binding_inv_known_fun f w ρ xs e :
+      K ! f = Some w ->
+      binding_inv f (Tag w (A1.Vfun f ρ xs e)).
+    Proof.
+      intros.
+      split; intros; simpl; auto.
+      rewrite H in H0; discriminate.
+    Qed.
+
+    Definition G i Γ1 ρ1 Γ2 ρ2 :=
+      wf_env ρ2 /\
+      forall x,
+        (x \in Γ1) ->
+        forall v1,
+          M.get x ρ1 = Some v1 ->
+          ((x \in Γ2) ->
+           exists v2,
+             M.get x ρ2 = Some v2 /\
+             binding_inv x v2 /\
+             V i v1 v2).
+
+    (* Environment Lemmas *)
+    Lemma G_subset Γ1 Γ2 {i ρ1 Γ3 ρ2 Γ4}:
+      G i Γ1 ρ1 Γ2 ρ2 ->
+      Γ3 \subset Γ1 ->
+      Γ4 \subset Γ2 ->
+      G i Γ3 ρ1 Γ4 ρ2.
+    Proof.
+      unfold G.
+      intros.
+      inv H; split; auto.
+    Qed.
+
+    Lemma G_wf_env_r {i Γ1 ρ1 Γ2 ρ2}:
+      G i Γ1 ρ1 Γ2 ρ2 ->
+      wf_env ρ2.
+    Proof.
+      unfold G.
+      intros H; destruct H; auto.
+    Qed.
+
+    Lemma G_get {Γ1 Γ2 i ρ1 ρ2}:
+      G i Γ1 ρ1 Γ2 ρ2 ->
+      forall x v1,
+        (x \in Γ1) ->
+        (x \in Γ2) ->
+        M.get x ρ1 = Some v1 ->
+        exists v2,
+          M.get x ρ2 = Some v2 /\
+          binding_inv x v2 /\
+          V i v1 v2.
+    Proof.
+      unfold G.
+      intros.
+      destruct H as [Hr1 HG].
+      eapply HG; eauto.
+    Qed.
+
+    Lemma G_get_list {i Γ1 ρ1 Γ2 ρ2} :
+      G i Γ1 ρ1 Γ2 ρ2 ->
+      forall xs vs1,
+        (FromList xs) \subset Γ1 ->
+        (FromList xs) \subset Γ2 ->
+        Disjoint _ (FromList xs) (Dom_map K) ->
+        get_list xs ρ1 = Some vs1 ->
+        exists vs2,
+          get_list xs ρ2 = Some vs2 /\
+          Forall exposed vs2 /\
+          Forall2 (V i) vs1 vs2.
+    Proof.
+      intros HG xs.
+      induction xs; simpl; intros.
+      - inv H2; eauto.
+      - destruct (ρ1 ! a) eqn:Heq1; try discriminate.
+        destruct (get_list xs ρ1) eqn:Heq3; try discriminate.
+        inv H2.
+        unfold Ensembles.Included, Ensembles.In in *.
+        edestruct (G_get HG) as [v2 [Heqv2 [[Hid HK] HV]]]; eauto.
+        eapply (H a).
+        apply in_eq.
+        apply H0.
+        apply in_eq.
+        edestruct IHxs as [vs2 [Heqvs2 [Hexvs2 Vvs]]]; eauto.
+        + intros.
+          apply H.
+          apply in_cons; auto.
+        + intros.
+          apply H0.
+          apply in_cons; auto.
+        + eapply Disjoint_FromList_cons_l; eauto.
+        + rewrite Heqvs2.
+          exists (v2 :: vs2); split; auto.
+          rewrite Heqv2; auto.
+          split; auto.
+          constructor; auto.
+          apply Disjoint_FromList_cons_inv in H1.
+          inv H1.
+          apply not_Dom_map_eq in H2; auto.
+    Qed.
+
+    Lemma G_set {i Γ1 ρ1 Γ2 ρ2}:
+      G i Γ1 ρ1 Γ2 ρ2 ->
+      forall {x v1 v2},
+        V i v1 v2 ->
+        binding_inv x v2 ->
+        G i (x |: Γ1) (M.set x v1 ρ1) (x |: Γ2) (M.set x v2 ρ2).
+    Proof.
+      intro HG.
+      pose proof HG as HG'.
+      unfold G in HG.
+      intros.
+
+      inv HG.
+      split.
+      eapply wf_env_set; eauto.
+      eapply V_wf_val_r; eauto.
+
+      intros.
+      destruct (M.elt_eq x0 x); subst.
+      - repeat rewrite M.gss in *.
+        inv H4.
+        eexists; repeat (split; intros; eauto).
+      - rewrite M.gso in *; auto.
+        eapply G_get; eauto.
+
+        inv H3; auto.
+        inv H6; try contradiction; auto.
+        inv H5; auto.
+        inv H6; try contradiction; auto.
+    Qed.
+
+    Lemma G_set_lists {i Γ1 ρ1 Γ2 ρ2}:
+      G i Γ1 ρ1 Γ2 ρ2 ->
+      forall {xs vs1 vs2 ρ3 ρ4},
+        Forall2 (V i) vs1 vs2 ->
+        Forall2 binding_inv xs vs2 ->
+        set_lists xs vs1 ρ1 = Some ρ3 ->
+        set_lists xs vs2 ρ2 = Some ρ4 ->
+        G i (FromList xs :|: Γ1) ρ3 (FromList xs :|: Γ2) ρ4.
+    Proof.
+      intros HG xs.
+      induction xs; simpl; intros.
+      - destruct vs1; try discriminate.
+        destruct vs2; try discriminate.
+        inv H1; inv H2.
+        eapply G_subset; eauto; normalize_sets;
+          rewrite Union_Empty_set_neut_l; eauto;
+          apply Included_refl.
+      - destruct vs1; try discriminate.
+        destruct vs2; try discriminate.
+        destruct (set_lists xs vs1 ρ1) eqn:Heq1; try discriminate.
+        destruct (set_lists xs vs2 ρ2) eqn:Heq2; try discriminate.
+        inv H; inv H0; inv H1; inv H2.
+        eapply G_subset with (Γ1 := (a |: (FromList xs :|: Γ1))) (Γ2 := (a |: (FromList xs :|: Γ2))); eauto;
+          try (normalize_sets;
+               rewrite Union_assoc;
+               apply Included_refl).
+        eapply G_set; eauto.
+    Qed.
+
+    (* Monotonicity Lemmas *)
+    Lemma V_mono_Forall_aux :
+      forall i j (V : nat -> A0.val -> A1.wval -> Prop) vs1 vs2,
+        (forall k : nat,
+            k < S i ->
+            forall (j : nat) v1 v2, V k v1 v2 -> j <= k -> V j v1 v2) ->
+        Forall2 (V i) vs1 vs2 ->
+        j <= i ->
+        Forall2 (V j) vs1 vs2.
+    Proof.
+      intros.
+      revert vs2 H0.
+      induction vs1; intros; inv H0; auto.
+      rename l' into vs2.
+      constructor; auto.
+      eapply H; eauto; lia.
+    Qed.
+
+    Lemma V_mono i :
+      forall {j v1 v2},
+        V i v1 v2 ->
+        j <= i ->
+        V j v1 v2.
+    Proof.
+      induction i using lt_wf_rec; intros.
+      destruct v2.
+      destruct i; simpl in H0;
+        destruct j; simpl; intros;
+        destruct H0 as [Hv1 HV]; subst.
+      - repeat (split; auto).
+      - inv H1.
+      - repeat (split; auto).
+        destruct v1; destruct v; try contradiction.
+        + destruct HV.
+          destruct (K ! v0) eqn:HeqK.
+          * destruct H2 as [Hlen [Heqw [Hex HV]]]; subst.
+            repeat (split; eauto).
+          * destruct H2 as [Hlen [Hex HV]].
+            repeat (split; eauto).
+        + destruct HV as [Hex [Hc HV]]; subst.
+          repeat split; auto.
+          eapply Forall2_length; eauto.
+      - repeat (split; auto).
+        destruct v1; destruct v; try contradiction.
+        + destruct HV as [Hf [Hlen HV]]; subst.
+          repeat split; auto.
+          destruct (K ! v) eqn:HeqK.
+          * destruct HV as [Heqw [Hex HV]]; subst.
+            repeat split; auto; intros.
+            specialize (HV j0 vs1 vs2 ρ3 ρ4).
+            rewrite normalize_step in *; try lia.
+            apply HV; eauto; lia.
+          * destruct HV as [Hex HV]; subst.
+            repeat split; auto; intros.
+            specialize (HV j0 vs1 vs2 ρ3 ρ4).
+            rewrite normalize_step in *; try lia.
+            eapply HV; eauto; lia.
+        + destruct HV as [Hex [Heqc HV]]; subst.
+          repeat split; auto.
+          eapply V_mono_Forall_aux; eauto; lia.
+    Qed.
+
+    Lemma V_mono_Forall {vs1 vs2} i j :
+      Forall2 (V i) vs1 vs2 ->
+      j <= i ->
+      Forall2 (V j) vs1 vs2.
+    Proof.
+      intros H.
+      revert j.
+      induction H; simpl; intros; auto.
+      constructor; eauto.
+      eapply V_mono; eauto.
+    Qed.
+
+    Lemma R_mono {r1 r2} i j :
+      R i r1 r2 ->
+      j <= i ->
+      R j r1 r2.
+    Proof.
+      unfold R.
+      intros.
+      destruct r1; auto.
+      destruct r2; auto.
+      eapply V_mono; eauto.
+    Qed.
+
+    Lemma E_mono {ex ρ1 ρ2 e1 e2} i j:
+      E ex i ρ1 e1 ρ2 e2 ->
+      j <= i ->
+      E ex j ρ1 e1 ρ2 e2.
+    Proof.
+      unfold E, R, E', R'.
+      intros.
+      destruct (H j1 r1) as [j2 [r2 [Hr2 HR]]]; auto; try lia.
+      exists j2, r2; split; eauto.
+      apply R_mono with (i - j1); try lia; auto.
+    Qed.
+
+    Lemma G_mono {Γ1 Γ2 ρ1 ρ2} i j:
+      G i Γ1 ρ1 Γ2 ρ2 ->
+      j <= i ->
+      G j Γ1 ρ1 Γ2 ρ2.
+    Proof.
+      unfold G.
+      intros.
+      inv H.
+      split; auto; intros.
+      edestruct H2 as [v2 [Heqv2 [[Hid HK] HV]]]; eauto.
+      eexists; eexists; repeat split; eauto.
+      apply V_mono with i; eauto.
+    Qed.
+
+    (* Compatibility Lemmas *)
+    Definition trans_correct Γ e1 e2 :=
+      forall i ρ1 ρ2,
+        known_map_inv K ->
+        G i Γ ρ1 (A1.occurs_free e2) ρ2 ->
+        E true i ρ1 e1 ρ2 e2.
+
+    Lemma ret_compat Γ x :
       (x \in Γ) ->
-      trans_ Γ (A0.Eret x) (A1.Eret x)
+      K ! x = None ->
+      trans_correct Γ (A0.Eret x) (A1.Eret x).
+    Proof.
+      unfold trans_correct, E, E', R, R', Ensembles.Included, Ensembles.In, Dom_map.
+      intros; simpl.
+      inv H4.
+      - exists 0, A1.OOT; split; auto.
+      - inv H5.
+        edestruct (G_get H2) as [v2 [Heqv2 [[Hid HK] HV]]]; eauto.
+        exists 1, (A1.Res v2); split; simpl; auto.
+        apply V_mono with i; try lia; auto.
+    Qed.
 
-  | Trans_fun_known :
-    forall {f w xs e k e' k'},
+    Lemma Vfun_V_known Γ1 f w xs e e' :
+      known_map_inv K ->
       K ! f = Some w ->
-      (~ w \in Exposed) ->
+      Disjoint _ (FromList xs) (Dom_map K) ->
+      trans_correct (FromList xs :|: (f |: Γ1)) e e' ->
+      forall {i Γ2 ρ1 ρ2},
+        wf_env ρ2 ->
+        G i Γ1 ρ1 Γ2 ρ2 ->
+        A1.occurs_free e' \subset (FromList xs :|: (f |: Γ2)) ->
+        V i (A0.Vfun f ρ1 xs e) (Tag w (A1.Vfun f ρ2 xs e')).
+    Proof.
+      unfold trans_correct.
+      intros HK HKf HKxs He i.
+      assert (~ Ensembles.In web Exposed w) by (eapply HK; eauto).
+      induction i; simpl; intros; auto;
+        rewrite HKf;
+        repeat (split; auto); intros.
+
+      apply (He (i - (i - j)) ρ3 ρ4); auto.
+      - eapply G_subset with (Γ2 := (FromList xs :|: (f |: Γ2))); eauto.
+        eapply G_set_lists; eauto.
+        eapply G_set; eauto.
+        + apply G_mono with (S i); eauto; lia.
+        + apply V_mono with i; try lia.
+          eapply IHi with (Γ2 := Γ2); eauto.
+          apply G_mono with (S i); eauto; lia.
+        + eapply binding_inv_known_fun; eauto.
+        + eapply binding_inv_exposed_Forall; eauto.
+          eapply set_lists_length_eq; eauto.
+        + apply Included_refl.
+    Qed.
+
+    Lemma fun_known_compat Γ e e' k k' f w xs :
+      K ! f = Some w ->
       Disjoint _ (FromList xs) (Dom_map K) ->
 
-      trans_ (FromList xs :|: (f |: Γ)) e e' ->
-      trans_ (f |: Γ) k k' ->
-      trans_ Γ (A0.Efun f xs e k) (A1.Efun f w xs e' k')
+      trans_correct (FromList xs :|: (f |: Γ)) e e' ->
+      trans_correct (f |: Γ) k k' ->
+      trans_correct Γ (A0.Efun f xs e k) (A1.Efun f w xs e' k').
+    Proof.
+      unfold trans_correct, E, E'.
+      intros HKf HKxs.
+      intros.
+      inv H4.
+      - exists 0, A1.OOT; split; simpl; eauto.
+      - inv H5.
+        edestruct (H0 (i - 1) (M.set f (A0.Vfun f ρ1 xs e) ρ1) (M.set f (Tag w (A1.Vfun f ρ2 xs e')) ρ2)) with (j1 := c) (r1 := r1) as [j2 [r2 [Hk2 Rr]]]; eauto; try lia.
+        + eapply G_subset with (Γ2 := (f |: A1.occurs_free (A1.Efun f w xs e' k'))).
+          eapply G_set; eauto.
+          apply G_mono with i; eauto; lia.
+          * eapply Vfun_V_known; eauto.
+            -- eapply G_wf_env_r; eauto.
+            -- apply G_mono with i; eauto; lia.
+            -- apply A1.free_fun_e_subset.
+          * eapply binding_inv_known_fun; eauto.
+          * apply Included_refl.
+          * apply A1.free_fun_k_subset.
+        + exists (S j2), r2; split; auto.
+          * constructor; simpl; auto.
+            eapply bstep_fuel_exposed_inv; eauto.
+          * apply R_mono with ((i - 1) - c); try lia; auto.
+    Qed.
 
-  | Trans_fun_unknown :
-    forall {f xs e k e' k'},
+    Lemma Vfun_V_unknown Γ1 f xs e e' :
+      known_map_inv K ->
+      K ! f = None ->
+      Disjoint _ (FromList xs) (Dom_map K) ->
+      trans_correct (FromList xs :|: (f |: Γ1)) e e' ->
+      forall {i Γ2 ρ1 ρ2},
+        wf_env ρ2 ->
+        G i Γ1 ρ1 Γ2 ρ2 ->
+        A1.occurs_free e' \subset (FromList xs :|: (f |: Γ2)) ->
+        V i (A0.Vfun f ρ1 xs e) (Tag w0 (A1.Vfun f ρ2 xs e')).
+    Proof.
+      unfold trans_correct.
+      intros HK HKf HKxs He i.
+      induction i; simpl; intros; auto;
+        rewrite HKf;
+        repeat (split; auto); intros;
+        try (constructor; apply w0_exposed).
+
+      apply (He (i - (i - j)) ρ3 ρ4); auto.
+      - eapply G_subset with (Γ2 := (FromList xs :|: (f |: Γ2))); eauto.
+        eapply G_set_lists; eauto.
+        eapply G_set; eauto.
+        + apply G_mono with (S i); eauto; lia.
+        + apply V_mono with i; try lia.
+          eapply IHi with (Γ2 := Γ2); eauto.
+          apply G_mono with (S i); eauto; lia.
+        + split; intros; simpl; auto.
+          constructor; apply w0_exposed.
+        + eapply binding_inv_exposed_Forall; eauto.
+          eapply set_lists_length_eq; eauto.
+        + apply Included_refl.
+    Qed.
+
+    Lemma fun_unknown_compat Γ e e' k k' f xs :
       K ! f = None ->
       Disjoint _ (FromList xs) (Dom_map K) ->
 
-      trans_ (FromList xs :|: (f |: Γ)) e e' ->
-      trans_ (f |: Γ) k k' ->
-      trans_ Γ (A0.Efun f xs e k) (A1.Efun f w0 xs e' k')
+      trans_correct (FromList xs :|: (f |: Γ)) e e' ->
+      trans_correct (f |: Γ) k k' ->
+      trans_correct Γ (A0.Efun f xs e k) (A1.Efun f w0 xs e' k').
+    Proof.
+      unfold trans_correct, E, E'.
+      intros HKf HKxs.
+      intros.
+      inv H4.
+      - exists 0, A1.OOT; split; simpl; eauto.
+      - inv H5.
+        edestruct (H0 (i - 1) (M.set f (A0.Vfun f ρ1 xs e) ρ1) (M.set f (Tag w0 (A1.Vfun f ρ2 xs e')) ρ2)) with (j1 := c) (r1 := r1) as [j2 [r2 [Hk2 Rr]]]; eauto; try lia.
+        + eapply G_subset with (Γ2 := (f |: A1.occurs_free (A1.Efun f w0 xs e' k'))).
+          eapply G_set; eauto.
+          apply G_mono with i; eauto; lia.
+          * eapply Vfun_V_unknown; eauto.
+            -- eapply G_wf_env_r; eauto.
+            -- apply G_mono with i; eauto; lia.
+            -- apply A1.free_fun_e_subset.
+          * eapply binding_inv_exposed; eauto.
+            constructor; apply w0_exposed.
+          * apply Included_refl.
+          * apply A1.free_fun_k_subset.
+        + exists (S j2), r2; split; auto.
+          * constructor; simpl; auto.
+            eapply bstep_fuel_exposed_inv; eauto.
+          * apply R_mono with ((i - 1) - c); try lia; auto.
+    Qed.
 
-  | Trans_app_known :
-    forall {f w xs},
-      K ! f = Some w ->
+    Lemma app_known_compat Γ xs f w :
+      (K ! f = Some w) ->
       (~ w \in Exposed) ->
       Disjoint _ (FromList xs) (Dom_map K) ->
 
       (f \in Γ) ->
       (FromList xs \subset Γ) ->
-      trans_ Γ (A0.Eapp f xs) (A1.Eapp f w xs)
+      trans_correct Γ (A0.Eapp f xs) (A1.Eapp f w xs).
+    Proof.
+      unfold trans_correct, E, E'.
+      intros HKf Hw HKxs.
+      intros; simpl.
 
-  | Trans_app_unknown :
-    forall {f xs},
-      K ! f = None ->
+      inv H4.
+      - exists 0, A1.OOT; split; simpl; auto.
+      - inv H5.
+        edestruct (G_get H2 f) as [fv2 [Heqfv2 [[Hid HK] HV]]]; eauto.
+        destruct i.
+        inv H3.
+        destruct fv2; simpl in HV;
+          destruct HV as [Hv1 HV];
+          destruct v; try contradiction.
+        specialize (Hid _ HKf).
+        apply same_id_fun in Hid; subst.
+        destruct HV as [Hfeq [Hlen HV]]; subst.
+        destruct (K ! f) eqn:Heqk; try contradiction.
+        + destruct HV as [Heqw [Hex HV]]; subst.
+          inv HKf.
+          clear HK Hex.
+
+          edestruct (G_get_list H2 xs vs) as [vs2 [Heqvs2 [Hexvs Vvs]]]; eauto.
+          eapply A1.free_app_xs_subset; eauto.
+
+          destruct (set_lists_length3 (M.set f (Tag w (A1.Vfun f t l e0)) t) l vs2) as [ρ4 Heqρ4].
+          unfold wval in *.
+          rewrite <- (Forall2_length _ _ _ Vvs).
+          rewrite <- (set_lists_length_eq _ _ _ _ H9); auto.
+
+          assert (HE : E true (i - (i - i)) ρ'' e ρ4 e0).
+          {
+            eapply (HV i vs vs2); eauto.
+            apply V_mono_Forall with (S i); auto; lia.
+          }
+
+          apply (E_mono _ i) in HE; try lia.
+          unfold E in HE.
+          destruct (HE c r1) as [j2 [r2 [He0 Rr]]]; try lia; auto.
+          exists (S j2), r2; split; eauto.
+          constructor; auto.
+          * econstructor; eauto.
+            destruct (exposed_reflect w); try contradiction; auto.
+            -- pose proof He0 as Hr2.
+               apply bstep_fuel_exposed_inv in Hr2.
+               eapply bstep_fuel_exposed; eauto.
+            -- intros; contradiction.
+          * eapply bstep_fuel_exposed_inv; eauto.
+        + destruct HV as [Hex HV].
+          inv Hex.
+          rewrite HKf in Heqk; discriminate.
+    Qed.
+
+    Lemma app_unknown_compat Γ xs f :
+      (K ! f = None) ->
       Disjoint _ (FromList xs) (Dom_map K) ->
 
       (f \in Γ) ->
       (FromList xs \subset Γ) ->
-      trans_ Γ (A0.Eapp f xs) (A1.Eapp f w0 xs)
+      trans_correct Γ (A0.Eapp f xs) (A1.Eapp f w0 xs).
+    Proof.
+      unfold trans_correct, E, E'.
+      intros HKf HKxs.
+      intros.
+      inv H4.
+      - exists 0, A1.OOT; split; simpl; auto.
+      - inv H5.
+        edestruct (G_get H2 f) as [fv2 [Heqfv2 [[Hid HK] HV]]]; eauto.
+        destruct i.
+        inv H3.
+        destruct fv2; simpl in HV;
+          destruct HV as [Hv1 HV];
+          destruct v; try contradiction.
+        destruct HV as [Hfeq [Hlen HV]]; subst.
+        rename v into f'.
+        destruct (K ! f') eqn:HeqKf'; try discriminate.
+        + destruct HV as [Heqw [Hex HV]]; subst.
+          specialize (HK HKf).
+          inv HK; contradiction.
+        + destruct HV as [Hex HV].
+          inv Hex.
+          assert (Hw : w = w0) by (apply Exposed_singleton; eauto); subst.
 
-  | Trans_letapp_known :
-    forall {x f w xs k k'},
+          edestruct (G_get_list H2 xs vs) as [vs2 [Heqvs2 [Hexvs Vvs]]]; eauto.
+          eapply A1.free_app_xs_subset; eauto.
+
+          destruct (set_lists_length3 (M.set f' (Tag w0 (A1.Vfun f' t l e0)) t) l vs2) as [ρ4 Heqρ4].
+          unfold wval in *.
+          rewrite <- (Forall2_length _ _ _ Vvs).
+          rewrite <- (set_lists_length_eq _ _ _ _ H9); auto.
+
+          assert (HE : E true (i - (i - i)) ρ'' e ρ4 e0).
+          {
+            eapply (HV i vs vs2); eauto.
+            apply V_mono_Forall with (S i); auto; lia.
+          }
+
+          apply (E_mono _ i) in HE; try lia.
+          unfold E in HE.
+          destruct (HE c r1) as [j2 [r2 [He0 Rr]]]; try lia; auto.
+          assert (exposed_res r2) by (eapply bstep_fuel_exposed_inv; eauto).
+          exists (S j2), r2; split; eauto; simpl.
+          constructor; auto.
+          econstructor; eauto.
+          destruct (exposed_reflect w0); try contradiction; auto.
+    Qed.
+
+    Lemma letapp_known_compat Γ k k' xs x w f :
       K ! f = Some w ->
       (~ w \in Exposed) ->
       Disjoint _ (FromList xs) (Dom_map K) ->
@@ -209,1789 +1065,897 @@ Section Known.
 
       (f \in Γ) ->
       (FromList xs \subset Γ) ->
-      trans_ (x |: Γ) k k' ->
-      trans_ Γ (A0.Eletapp x f xs k) (A1.Eletapp x f w xs k')
+      trans_correct (x |: Γ) k k' ->
+      trans_correct Γ (A0.Eletapp x f xs k) (A1.Eletapp x f w xs k').
+    Proof.
+      intros HKf Hw HKxs HKx.
+      intros.
+      specialize (app_known_compat Γ xs f w HKf Hw HKxs H H0); intros Ha.
+      unfold trans_correct, E, E' in *.
+      intros.
 
-  | Trans_letapp_unknown :
-    forall {x f xs k k'},
+      assert (HG' : G i Γ ρ1 (occurs_free (A1.Eapp f w xs)) ρ2).
+      {
+        eapply G_subset with (Γ2 := (occurs_free (A1.Eletapp x f w xs k'))); eauto.
+        apply Included_refl.
+        eapply free_app_letapp; eauto.
+      }
+
+      inv H5.
+      - exists 0, OOT; split; simpl; auto.
+      - inv H6.
+        + destruct (Ha i ρ1 ρ2) with (j1 := (S c0)) (r1 := (A0.Res v)) as [j2 [r2 [Hr1 HR]]]; try lia; eauto.
+          * simpl in HR.
+            destruct r2; try contradiction.
+            rename w1 into v0.
+            inv Hr1.
+
+            edestruct (H1 (i - (S c0)) (M.set x v ρ1) (M.set x v0 ρ2)) with (j1 := c') as [j2 [r2 [Hk Rr]]]; eauto; try lia.
+            -- eapply G_subset with (Γ2 := (x |: (A1.occurs_free (A1.Eletapp x f w xs k')))).
+               eapply G_set; eauto.
+               apply G_mono with i; try lia; eauto.
+               eapply binding_inv_exposed; eauto.
+               inv H6; auto.
+               apply Included_refl.
+               apply free_letapp_k_subset.
+            -- exists ((S c) + j2), r2; split.
+               ++ inv H5.
+                  rewrite_math ((S c + j2) = S (c + j2)).
+                  constructor; auto.
+                  ** eapply BStep_letapp_Res; eauto.
+                     intros.
+                     destruct H21; auto.
+                     inv H8.
+                     split; auto.
+                  ** eapply bstep_fuel_exposed_inv; eauto.
+               ++ apply R_mono with (i - S c0 - c'); try lia; auto.
+        + eexists; eexists; repeat split; eauto.
+          simpl; auto.
+    Qed.
+
+    Lemma letapp_unknown_compat Γ k k' xs x f :
       K ! f = None ->
       Disjoint _ (FromList xs) (Dom_map K) ->
       K ! x = None ->
 
       (f \in Γ) ->
       (FromList xs \subset Γ) ->
-      trans_ (x |: Γ) k k' ->
-      trans_ Γ (A0.Eletapp x f xs k) (A1.Eletapp x f w0 xs k')
+      trans_correct (x |: Γ) k k' ->
+      trans_correct Γ (A0.Eletapp x f xs k) (A1.Eletapp x f w0 xs k').
+    Proof.
+      intros HKf HKxs HKx.
+      intros.
+      specialize (app_unknown_compat Γ xs f HKf HKxs H H0); intros Ha.
+      unfold trans_correct, E, E' in *.
+      intros.
 
-  (* data webs are all exposed *)
+      assert (HG' : G i Γ ρ1 (occurs_free (A1.Eapp f w0 xs)) ρ2).
+      {
+        eapply G_subset with (Γ2 := (occurs_free (A1.Eletapp x f w0 xs k'))); eauto.
+        apply Included_refl.
+        eapply free_app_letapp; eauto.
+      }
 
-  | Trans_constr :
-    forall {x t xs k k'},
+      inv H5.
+      - exists 0, OOT; split; simpl; auto.
+      - inv H6.
+        + destruct (Ha i ρ1 ρ2) with (j1 := (S c0)) (r1 := (A0.Res v)) as [j2 [r2 [Hr1 HR]]]; try lia; eauto.
+          * simpl in HR.
+            destruct r2; try contradiction.
+            rename w into v0.
+            inv Hr1.
+
+            edestruct (H1 (i - (S c0)) (M.set x v ρ1) (M.set x v0 ρ2)) with (j1 := c') as [j2 [r2 [Hk Rr]]]; eauto; try lia.
+            -- eapply G_subset with (Γ2 := (x |: (A1.occurs_free (A1.Eletapp x f w0 xs k')))).
+               eapply G_set; eauto.
+               apply G_mono with i; try lia; eauto.
+               eapply binding_inv_exposed; eauto.
+               inv H6; auto.
+               apply Included_refl.
+               apply free_letapp_k_subset.
+            -- exists ((S c) + j2), r2; split.
+               ++ inv H5.
+                  rewrite_math ((S c + j2) = S (c + j2)).
+                  constructor; auto.
+                  ** eapply BStep_letapp_Res; eauto.
+                     intros.
+                     destruct H21; auto.
+                     inv H8.
+                     split; auto.
+                  ** eapply bstep_fuel_exposed_inv; eauto.
+               ++ apply R_mono with (i - S c0 - c'); try lia; auto.
+        + eexists; eexists; repeat split; eauto.
+          simpl; auto.
+    Qed.
+
+    Lemma constr_compat Γ x t xs k k' :
       K ! x = None ->
       Disjoint _ (FromList xs) (Dom_map K) ->
 
       (FromList xs \subset Γ) ->
-      trans_ (x |: Γ) k k' ->
-      trans_ Γ (A0.Econstr x t xs k) (A1.Econstr x w0 t xs k')
+      trans_correct (x |: Γ) k k' ->
+      trans_correct Γ (A0.Econstr x t xs k) (A1.Econstr x w0 t xs k').
+    Proof.
+      unfold trans_correct, E, E'.
+      intros.
+      inv H6.
+      - exists 0, A1.OOT; split; simpl; auto.
+      - inv H7.
+        destruct (G_get_list H4 xs vs) as [vs' [Heqvs' Hvs]]; auto.
+        + eapply A1.free_constr_xs_subset; eauto.
+        + inv Hvs.
+          assert (wf_val (Tag w0 (A1.Vconstr t vs'))).
+          {
+            apply wf_val_Vconstr; auto.
+            eapply V_wf_val_Forall_r; eauto.
+          }
 
-  | Trans_proj :
-    forall {x y k k' n},
+          assert (exposed (Tag w0 (A1.Vconstr t vs'))).
+          {
+            constructor; auto.
+            apply w0_exposed.
+          }
+
+          assert (length vs = length vs').
+          {
+            unfold wval in *.
+            rewrite <- (get_list_length_eq _ _ _ H13).
+            rewrite <- (get_list_length_eq _ _ _ Heqvs'); auto.
+          }
+
+          edestruct (H2 i (M.set x (A0.Vconstr t vs) ρ1) (M.set x (Tag w0 (A1.Vconstr t vs')) ρ2)) with (j1 := c) (r1 := r1) as [j2 [r2 [Hk' Rr]]]; eauto; try lia.
+          * eapply G_subset with (Γ2 := (x |: (A1.occurs_free (A1.Econstr x w0 t xs k')))).
+            eapply G_set; eauto.
+            -- destruct i; simpl; repeat (split; eauto).
+               eapply V_mono_Forall; eauto; lia.
+            -- eapply binding_inv_exposed; eauto.
+            -- apply Included_refl.
+            -- apply A1.free_constr_k_subset.
+          * exists (S j2), r2; split; eauto.
+            -- econstructor.
+               econstructor; eauto.
+               eapply bstep_fuel_exposed_inv in Hk'; eauto.
+            -- apply R_mono with (i - c); try lia; auto.
+    Qed.
+
+    Lemma proj_compat Γ x i y e e' :
       K ! x = None ->
       K ! y = None ->
 
       (y \in Γ) ->
-      trans_ (x |: Γ) k k' ->
-      trans_ Γ (A0.Eproj x n y k) (A1.Eproj x w0 n y k')
-
-  | Trans_case_nil :
-    forall {x},
-      K ! x = None ->
-      (x \in Γ) ->
-      trans_ Γ (A0.Ecase x []) (A1.Ecase x w0 [])
-
-  | Trans_case_cons :
-    forall {x e e' t cl cl'},
-      K ! x = None ->
-      (x \in Γ) ->
-      trans_ Γ e e' ->
-      trans_ Γ (A0.Ecase x cl) (A1.Ecase x w0 cl') ->
-      trans_ Γ (A0.Ecase x ((t, e) :: cl)) (A1.Ecase x w0 ((t, e') :: cl')).
-
-  Hint Constructors trans_ : core.
-
-  Definition trans := trans_.
-
-  Hint Unfold trans : core.
-
-  Lemma known_fun_trans e :
-    known_map_inv K ->
-    known_fun (Dom_map K) e ->
-    forall Γ,
-      (A0.occurs_free e) \subset Γ ->
-      exists e', trans Γ e e'.
-  Proof.
-    unfold known_map_inv.
-    intros HK H.
-    induction H; simpl; intros.
-    - exists (A1.Eret x); auto.
-    - apply Dom_map_eq in H.
-      destruct H as [w Hw].
-      exists (A1.Eapp f w ys); econstructor; eauto.
-      eapply A0.free_app_xs_inv; eauto.
-    - apply Dom_map_eq in H.
-      destruct H as [w Hw].
-      destruct (IHknown_fun (x |: Γ)) as [e' He']; auto.
-      eapply A0.free_letapp_k_inv; eauto.
-      exists (A1.Eletapp x f w ys e'); econstructor; eauto.
-      eapply A0.free_letapp_xs_inv; eauto.
-    - apply Dom_map_eq in H.
-      destruct H as [w Hw].
-      destruct (IHknown_fun1 (FromList xs :|: (f |: Γ))) as [e' He']; auto.
-      eapply A0.free_fun_e_inv; eauto.
-      destruct (IHknown_fun2 (f |: Γ)) as [k' Hk']; auto.
-      eapply A0.free_fun_k_inv; eauto.
-      exists (A1.Efun f w xs e' k'); econstructor; eauto.
-    - destruct (IHknown_fun (x |: Γ)) as [e' He']; auto.
-      eapply A0.free_constr_k_inv; eauto.
-      exists (A1.Econstr x w0 ct ys e'); econstructor; eauto.
-      eapply A0.free_constr_xs_inv; eauto.
-    - destruct (IHknown_fun (x |: Γ)) as [e' He']; auto.
-      eapply A0.free_proj_k_inv; eauto.
-      exists (A1.Eproj x w0 n y e'); econstructor; eauto.
-    - exists (A1.Ecase x w0 []); econstructor; eauto.
-    - destruct (IHknown_fun1 Γ) as [e' He']; auto.
-      eapply A0.free_case_hd_inv; eauto.
-      destruct (IHknown_fun2 Γ) as [c' Hc']; auto.
-      eapply A0.free_case_tl_inv; eauto.
-      inv Hc'.
-      + exists (A1.Ecase x w0 [(c, e')]); econstructor; eauto.
-      + exists (A1.Ecase x w0 ((c, e') :: (t, e'0) :: cl')); econstructor; eauto.
-  Qed.
-
-  Corollary known_fun_trans_total e :
-    known_map_inv K ->
-    known_fun (Dom_map K) e ->
-    exists e', trans (A0.occurs_free e) e e'.
-  Proof.
-    intros.
-    eapply known_fun_trans; eauto.
-    apply Included_refl.
-  Qed.
-
-  Lemma trans_exp_inv {Γ e e'} :
-    trans Γ e e' ->
-    (A1.occurs_free e') \subset (A0.occurs_free e).
-  Proof.
-    unfold Ensembles.Included, Ensembles.In.
-    intros H.
-    induction H; simpl; intros; auto.
-    - inv H1; auto.
-    - inv H4; auto.
-    - inv H3; auto.
-    - inv H4; auto.
-    - inv H3; auto.
-    - inv H6; auto.
-    - inv H5; auto.
-    - inv H3; auto.
-    - inv H3; auto.
-    - inv H1; auto.
-    - inv H3; auto.
-  Qed.
-
-  Lemma Erase_Annotate_id e1 e2 e1' :
-    trans (A0.occurs_free e1) e1 e1' ->
-    Erase.trans (A1.occurs_free e1') e1' e2 ->
-    e1 = e2.
-  Proof.
-    unfold trans.
-    intro H.
-    revert e2.
-    induction H; simpl; intros.
-    - inv H1; auto.
-    - inv H4; auto.
-      erewrite IHtrans_1 with (e2 := e'0); eauto.
-      + erewrite IHtrans_2 with (e2 := k'0); eauto.
-        eapply Erase.trans_exp_strengthen; eauto.
-        eapply A1.free_fun_k_subset; eauto.
-      + eapply Erase.trans_exp_strengthen; eauto.
-        eapply A1.free_fun_e_subset; eauto.
-    - inv H3; auto.
-      erewrite IHtrans_1 with (e2 := e'0); eauto.
-      + erewrite IHtrans_2 with (e2 := k'0); eauto.
-        eapply Erase.trans_exp_strengthen; eauto.
-        eapply A1.free_fun_k_subset; eauto.
-      + eapply Erase.trans_exp_strengthen; eauto.
-        eapply A1.free_fun_e_subset; eauto.
-    - inv H4; auto.
-    - inv H3; auto.
-    - inv H6; auto.
-      erewrite IHtrans_ with (e2 := k'0); eauto.
-      eapply Erase.trans_exp_strengthen; eauto.
-      eapply A1.free_letapp_k_subset; eauto.
-    - inv H5; auto.
-      erewrite IHtrans_ with (e2 := k'0); eauto.
-      eapply Erase.trans_exp_strengthen; eauto.
-      eapply A1.free_letapp_k_subset; eauto.
-    - inv H3; auto.
-      erewrite IHtrans_ with (e2 := k'0); eauto.
-      eapply Erase.trans_exp_strengthen; eauto.
-      eapply A1.free_constr_k_subset; eauto.
-    - inv H3; auto.
-      erewrite IHtrans_ with (e2 := k'0); eauto.
-      eapply Erase.trans_exp_strengthen; eauto.
-      eapply A1.free_proj_k_subset; eauto.
-    - inv H1; auto.
-    - inv H3; auto.
-      erewrite IHtrans_1 with (e2 := e'0); eauto.
-      assert (A0.Ecase x cl = A0.Ecase x cl'0).
-      {
-        erewrite IHtrans_2 with (e2 := (A0.Ecase x cl'0)); eauto.
-        eapply Erase.trans_exp_strengthen; eauto.
-        eapply A1.free_case_tl_subset; eauto.
-      }
-      inv H3; auto.
-      eapply Erase.trans_exp_strengthen; eauto.
-      eapply A1.free_case_hd_subset; eauto.
-  Qed.
-
-  (* Cross-language Logical Relations *)
-  (* Note these are parameterized by the known_map, `K` *)
-  Definition R' (P : nat -> A0.val -> A1.wval -> Prop) (i : nat) (r1 : A0.res) (r2 : A1.res) :=
-    match r1, r2 with
-    | A0.OOT, A1.OOT => True
-    | A0.Res v1, A1.Res v2 => P i v1 v2
-    | _, _ => False
-    end.
-
-  Definition E' (P : nat -> A0.val -> A1.wval -> Prop) (ex : bool) (i : nat) (ρ1 : A0.env) (e1 :A0.exp) (ρ2 : A1.env) (e2 : A1.exp) : Prop :=
-    forall j1 r1,
-      j1 <= i ->
-      A0.bstep_fuel ρ1 e1 j1 r1 ->
-      exists j2 r2,
-        A1.bstep_fuel ex ρ2 e2 j2 r2 /\
-        R' P (i - j1) r1 r2.
-
-  Fixpoint V (i : nat) (v1 : A0.val) (wv2 : A1.wval) {struct i} : Prop :=
-    wf_val wv2 /\
-    match wv2 with
-    | A1.TAG _ w2 v2 =>
-        match v1, v2 with
-        | A0.Vconstr c1 vs1, A1.Vconstr c2 vs2 =>
-            exposed wv2 /\
-            c1 = c2 /\
-            match i with
-            | 0 => length vs1 = length vs2
-            | S i0 => Forall2 (V i0) vs1 vs2
-            end
-
-        | A0.Vfun f1 ρ1 xs1 e1, A1.Vfun f2 ρ2 xs2 e2 =>
-            (* note function arguments and result are always exposed regardless of whether a function is known or unknown *)
-            f1 = f2 /\
-            length xs1 = length xs2 /\
-            match K ! f1 with
-            | None => (* unknown *)
-                exposed wv2 /\
-                match i with
-                | 0 => True
-                | S i0 =>
-                    forall j vs1 vs2 ρ3 ρ4,
-                      j <= i0 ->
-                      Forall exposed vs2 ->
-                      Forall2 (V (i0 - (i0 - j))) vs1 vs2 ->
-                      set_lists xs1 vs1 (M.set f1 (A0.Vfun f1 ρ1 xs1 e1) ρ1) = Some ρ3 ->
-                      set_lists xs2 vs2 (M.set f2 (Tag w2 (A1.Vfun f2 ρ2 xs2 e2)) ρ2) = Some ρ4 ->
-                      E' V true (i0 - (i0 - j)) ρ3 e1 ρ4 e2
-                end
-            | Some w1 => (* known *)
-                w1 = w2 /\
-                (~ w1 \in Exposed) /\
-                match i with
-                | 0 => True
-                | S i0 =>
-                    forall j vs1 vs2 ρ3 ρ4,
-                      j <= i0 ->
-                      Forall exposed vs2 ->
-                      Forall2 (V (i0 - (i0 - j))) vs1 vs2 ->
-                      set_lists xs1 vs1 (M.set f1 (A0.Vfun f1 ρ1 xs1 e1) ρ1) = Some ρ3 ->
-                      set_lists xs2 vs2 (M.set f2 (Tag w2 (A1.Vfun f2 ρ2 xs2 e2)) ρ2) = Some ρ4 ->
-                      E' V true (i0 - (i0 - j)) ρ3 e1 ρ4 e2
-                end
-            end
-        | _, _ => False
-        end
-    end.
-
-  Definition R := (R' V).
-
-  Definition E := (E' V).
-
-  (* Lemmas about [wf_val], [wf_res], and [wf_env] *)
-  Lemma V_wf_val_r {i v1 v2}:
-    V i v1 v2 ->
-    wf_val v2.
-  Proof.
-    intros HV.
-    destruct i; simpl in *;
-      destruct HV as [Hv2 _]; auto.
-  Qed.
-
-  Lemma V_wf_val_Forall_r {i vs1 vs2} :
-    Forall2 (V i) vs1 vs2 ->
-    Forall wf_val vs2.
-  Proof.
-    intros.
-    induction H; auto.
-    constructor; auto.
-    eapply V_wf_val_r; eauto.
-  Qed.
-
-  Lemma V_wf_res_r {i v1 v2}:
-    V i v1 v2 ->
-    wf_res (Res v2).
-  Proof.
-    intros HV.
-    constructor.
-    eapply V_wf_val_r; eauto.
-  Qed.
-
-  Lemma R_wf_res_l {i r1 r2} :
-    R i r1 r2 ->
-    wf_res r2.
-  Proof.
-    unfold R.
-    intros.
-    destruct r1; destruct r2; try contradiction; auto.
-    constructor.
-    eapply V_wf_val_r; eauto.
-  Qed.
-
-  (* Inversion Lemmas *)
-  Lemma R_res_inv_l i v1 r2 :
-    R i (A0.Res v1) r2 ->
-    exists v2, r2 = A1.Res v2 /\ V i v1 v2.
-  Proof.
-    intros.
-    destruct r2; simpl in *; try contradiction.
-    eexists; split; eauto.
-  Qed.
-
-  (* Environment Relation *)
-  Definition same_id x wv2 :=
-    match wv2 with
-    | A1.TAG _ w2 v2 =>
-        match v2 with
-        | A1.Vfun f2 ρ2 xs2 e2 => f2 = x
-        | A1.Vconstr c2 vs2 => True
-        end
-    end.
-
-  Lemma same_id_fun f w f1 t l e:
-    same_id f (TAG val w (Vfun f1 t l e)) -> f1 = f.
-  Proof. unfold same_id; simpl; auto. Qed.
-
-  Definition binding_inv x v :=
-    (forall w, K ! x = Some w -> same_id x v) /\
-    (K ! x = None -> exposed v).
-
-  Lemma binding_inv_exposed x v :
-    (K ! x = None) ->
-    exposed v ->
-    binding_inv x v.
-  Proof.
-    unfold binding_inv.
-    intros.
-    split; intros; auto.
-    rewrite H in H1; discriminate.
-  Qed.
-
-  Lemma binding_inv_exposed_Forall xs :
-    forall vs,
-      Disjoint _ (FromList xs) (Dom_map K) ->
-      length xs = length vs ->
-      Forall exposed vs ->
-      Forall2 binding_inv xs vs.
-  Proof.
-    induction xs; simpl; intros;
-      destruct vs; try discriminate; auto.
-    inv H1.
-    apply Disjoint_FromList_cons_inv in H.
-    inv H.
-    constructor; auto.
-    apply binding_inv_exposed; auto.
-  Qed.
-
-  Lemma binding_inv_known_fun f w ρ xs e :
-    K ! f = Some w ->
-    binding_inv f (Tag w (A1.Vfun f ρ xs e)).
-  Proof.
-    intros.
-    split; intros; simpl; auto.
-    rewrite H in H0; discriminate.
-  Qed.
-
-  Definition G i Γ1 ρ1 Γ2 ρ2 :=
-    wf_env ρ2 /\
-    forall x,
-      (x \in Γ1) ->
-      forall v1,
-        M.get x ρ1 = Some v1 ->
-        ((x \in Γ2) ->
-         exists v2,
-           M.get x ρ2 = Some v2 /\
-           binding_inv x v2 /\
-           V i v1 v2).
-
-  (* Environment Lemmas *)
-  Lemma G_subset Γ1 Γ2 {i ρ1 Γ3 ρ2 Γ4}:
-    G i Γ1 ρ1 Γ2 ρ2 ->
-    Γ3 \subset Γ1 ->
-    Γ4 \subset Γ2 ->
-    G i Γ3 ρ1 Γ4 ρ2.
-  Proof.
-    unfold G.
-    intros.
-    inv H; split; auto.
-  Qed.
-
-  Lemma G_wf_env_r {i Γ1 ρ1 Γ2 ρ2}:
-    G i Γ1 ρ1 Γ2 ρ2 ->
-    wf_env ρ2.
-  Proof.
-    unfold G.
-    intros H; destruct H; auto.
-  Qed.
-
-  Lemma G_get {Γ1 Γ2 i ρ1 ρ2}:
-    G i Γ1 ρ1 Γ2 ρ2 ->
-    forall x v1,
-      (x \in Γ1) ->
-      (x \in Γ2) ->
-      M.get x ρ1 = Some v1 ->
-      exists v2,
-        M.get x ρ2 = Some v2 /\
-        binding_inv x v2 /\
-        V i v1 v2.
-  Proof.
-    unfold G.
-    intros.
-    destruct H as [Hr1 HG].
-    eapply HG; eauto.
-  Qed.
-
-  Lemma G_get_list {i Γ1 ρ1 Γ2 ρ2} :
-    G i Γ1 ρ1 Γ2 ρ2 ->
-    forall xs vs1,
-      (FromList xs) \subset Γ1 ->
-      (FromList xs) \subset Γ2 ->
-      Disjoint _ (FromList xs) (Dom_map K) ->
-      get_list xs ρ1 = Some vs1 ->
-      exists vs2,
-        get_list xs ρ2 = Some vs2 /\
-        Forall exposed vs2 /\
-        Forall2 (V i) vs1 vs2.
-  Proof.
-    intros HG xs.
-    induction xs; simpl; intros.
-    - inv H2; eauto.
-    - destruct (ρ1 ! a) eqn:Heq1; try discriminate.
-      destruct (get_list xs ρ1) eqn:Heq3; try discriminate.
-      inv H2.
-      unfold Ensembles.Included, Ensembles.In in *.
-      edestruct (G_get HG) as [v2 [Heqv2 [[Hid HK] HV]]]; eauto.
-      eapply (H a).
-      apply in_eq.
-      apply H0.
-      apply in_eq.
-      edestruct IHxs as [vs2 [Heqvs2 [Hexvs2 Vvs]]]; eauto.
-      + intros.
-        apply H.
-        apply in_cons; auto.
-      + intros.
-        apply H0.
-        apply in_cons; auto.
-      + eapply Disjoint_FromList_cons_l; eauto.
-      + rewrite Heqvs2.
-        exists (v2 :: vs2); split; auto.
-        rewrite Heqv2; auto.
-        split; auto.
-        constructor; auto.
-        apply Disjoint_FromList_cons_inv in H1.
-        inv H1.
-        apply not_Dom_map_eq in H2; auto.
-  Qed.
-
-  Lemma G_set {i Γ1 ρ1 Γ2 ρ2}:
-    G i Γ1 ρ1 Γ2 ρ2 ->
-    forall {x v1 v2},
-      V i v1 v2 ->
-      binding_inv x v2 ->
-      G i (x |: Γ1) (M.set x v1 ρ1) (x |: Γ2) (M.set x v2 ρ2).
-  Proof.
-    intro HG.
-    pose proof HG as HG'.
-    unfold G in HG.
-    intros.
-
-    inv HG.
-    split.
-    eapply wf_env_set; eauto.
-    eapply V_wf_val_r; eauto.
-
-    intros.
-    destruct (M.elt_eq x0 x); subst.
-    - repeat rewrite M.gss in *.
-      inv H4.
-      eexists; repeat (split; intros; eauto).
-    - rewrite M.gso in *; auto.
-      eapply G_get; eauto.
-
-      inv H3; auto.
-      inv H6; try contradiction; auto.
-      inv H5; auto.
-      inv H6; try contradiction; auto.
-  Qed.
-
-  Lemma G_set_lists {i Γ1 ρ1 Γ2 ρ2}:
-    G i Γ1 ρ1 Γ2 ρ2 ->
-    forall {xs vs1 vs2 ρ3 ρ4},
-      Forall2 (V i) vs1 vs2 ->
-      Forall2 binding_inv xs vs2 ->
-      set_lists xs vs1 ρ1 = Some ρ3 ->
-      set_lists xs vs2 ρ2 = Some ρ4 ->
-      G i (FromList xs :|: Γ1) ρ3 (FromList xs :|: Γ2) ρ4.
-  Proof.
-    intros HG xs.
-    induction xs; simpl; intros.
-    - destruct vs1; try discriminate.
-      destruct vs2; try discriminate.
-      inv H1; inv H2.
-      eapply G_subset; eauto; normalize_sets;
-        rewrite Union_Empty_set_neut_l; eauto;
-        apply Included_refl.
-    - destruct vs1; try discriminate.
-      destruct vs2; try discriminate.
-      destruct (set_lists xs vs1 ρ1) eqn:Heq1; try discriminate.
-      destruct (set_lists xs vs2 ρ2) eqn:Heq2; try discriminate.
-      inv H; inv H0; inv H1; inv H2.
-      eapply G_subset with (Γ1 := (a |: (FromList xs :|: Γ1))) (Γ2 := (a |: (FromList xs :|: Γ2))); eauto;
-        try (normalize_sets;
-             rewrite Union_assoc;
-             apply Included_refl).
-      eapply G_set; eauto.
-  Qed.
-
-  (* Monotonicity Lemmas *)
-  Lemma V_mono_Forall_aux :
-    forall i j (V : nat -> A0.val -> A1.wval -> Prop) vs1 vs2,
-      (forall k : nat,
-          k < S i ->
-          forall (j : nat) v1 v2, V k v1 v2 -> j <= k -> V j v1 v2) ->
-      Forall2 (V i) vs1 vs2 ->
-      j <= i ->
-      Forall2 (V j) vs1 vs2.
-  Proof.
-    intros.
-    revert vs2 H0.
-    induction vs1; intros; inv H0; auto.
-    rename l' into vs2.
-    constructor; auto.
-    eapply H; eauto; lia.
-  Qed.
-
-  Lemma V_mono i :
-    forall {j v1 v2},
-      V i v1 v2 ->
-      j <= i ->
-      V j v1 v2.
-  Proof.
-    induction i using lt_wf_rec; intros.
-    destruct v2.
-    destruct i; simpl in H0;
-      destruct j; simpl; intros;
-      destruct H0 as [Hv1 HV]; subst.
-    - repeat (split; auto).
-    - inv H1.
-    - repeat (split; auto).
-      destruct v1; destruct v; try contradiction.
-      + destruct HV.
-        destruct (K ! v0) eqn:HeqK.
-        * destruct H2 as [Hlen [Heqw [Hex HV]]]; subst.
-          repeat (split; eauto).
-        * destruct H2 as [Hlen [Hex HV]].
-          repeat (split; eauto).
-      + destruct HV as [Hex [Hc HV]]; subst.
-        repeat split; auto.
-        eapply Forall2_length; eauto.
-    - repeat (split; auto).
-      destruct v1; destruct v; try contradiction.
-      + destruct HV as [Hf [Hlen HV]]; subst.
-        repeat split; auto.
-        destruct (K ! v) eqn:HeqK.
-        * destruct HV as [Heqw [Hex HV]]; subst.
-          repeat split; auto; intros.
-          specialize (HV j0 vs1 vs2 ρ3 ρ4).
-          rewrite normalize_step in *; try lia.
-          apply HV; eauto; lia.
-        * destruct HV as [Hex HV]; subst.
-          repeat split; auto; intros.
-          specialize (HV j0 vs1 vs2 ρ3 ρ4).
-          rewrite normalize_step in *; try lia.
-          eapply HV; eauto; lia.
-      + destruct HV as [Hex [Heqc HV]]; subst.
-        repeat split; auto.
-        eapply V_mono_Forall_aux; eauto; lia.
-  Qed.
-
-  Lemma V_mono_Forall {vs1 vs2} i j :
-    Forall2 (V i) vs1 vs2 ->
-    j <= i ->
-    Forall2 (V j) vs1 vs2.
-  Proof.
-    intros H.
-    revert j.
-    induction H; simpl; intros; auto.
-    constructor; eauto.
-    eapply V_mono; eauto.
-  Qed.
-
-  Lemma R_mono {r1 r2} i j :
-    R i r1 r2 ->
-    j <= i ->
-    R j r1 r2.
-  Proof.
-    unfold R.
-    intros.
-    destruct r1; auto.
-    destruct r2; auto.
-    eapply V_mono; eauto.
-  Qed.
-
-  Lemma E_mono {ex ρ1 ρ2 e1 e2} i j:
-    E ex i ρ1 e1 ρ2 e2 ->
-    j <= i ->
-    E ex j ρ1 e1 ρ2 e2.
-  Proof.
-    unfold E, R, E', R'.
-    intros.
-    destruct (H j1 r1) as [j2 [r2 [Hr2 HR]]]; auto; try lia.
-    exists j2, r2; split; eauto.
-    apply R_mono with (i - j1); try lia; auto.
-  Qed.
-
-  Lemma G_mono {Γ1 Γ2 ρ1 ρ2} i j:
-    G i Γ1 ρ1 Γ2 ρ2 ->
-    j <= i ->
-    G j Γ1 ρ1 Γ2 ρ2.
-  Proof.
-    unfold G.
-    intros.
-    inv H.
-    split; auto; intros.
-    edestruct H2 as [v2 [Heqv2 [[Hid HK] HV]]]; eauto.
-    eexists; eexists; repeat split; eauto.
-    apply V_mono with i; eauto.
-  Qed.
-
-  (* Compatibility Lemmas *)
-  Definition trans_correct Γ e1 e2 :=
-    forall i ρ1 ρ2,
-      known_map_inv K ->
-      G i Γ ρ1 (A1.occurs_free e2) ρ2 ->
-      E true i ρ1 e1 ρ2 e2.
-
-  Lemma ret_compat Γ x :
-    (x \in Γ) ->
-    K ! x = None ->
-    trans_correct Γ (A0.Eret x) (A1.Eret x).
-  Proof.
-    unfold trans_correct, E, E', R, R', Ensembles.Included, Ensembles.In, Dom_map.
-    intros; simpl.
-    inv H4.
-    - exists 0, A1.OOT; split; auto.
-    - inv H5.
-      edestruct (G_get H2) as [v2 [Heqv2 [[Hid HK] HV]]]; eauto.
-      exists 1, (A1.Res v2); split; simpl; auto.
-      apply V_mono with i; try lia; auto.
-  Qed.
-
-  Lemma Vfun_V_known Γ1 f w xs e e' :
-    known_map_inv K ->
-    K ! f = Some w ->
-    Disjoint _ (FromList xs) (Dom_map K) ->
-    trans_correct (FromList xs :|: (f |: Γ1)) e e' ->
-    forall {i Γ2 ρ1 ρ2},
-      wf_env ρ2 ->
-      G i Γ1 ρ1 Γ2 ρ2 ->
-      A1.occurs_free e' \subset (FromList xs :|: (f |: Γ2)) ->
-      V i (A0.Vfun f ρ1 xs e) (Tag w (A1.Vfun f ρ2 xs e')).
-  Proof.
-    unfold trans_correct.
-    intros HK HKf HKxs He i.
-    assert (~ Ensembles.In web Exposed w) by (eapply HK; eauto).
-    induction i; simpl; intros; auto;
-      rewrite HKf;
-      repeat (split; auto); intros.
-
-    apply (He (i - (i - j)) ρ3 ρ4); auto.
-    - eapply G_subset with (Γ2 := (FromList xs :|: (f |: Γ2))); eauto.
-      eapply G_set_lists; eauto.
-      eapply G_set; eauto.
-      + apply G_mono with (S i); eauto; lia.
-      + apply V_mono with i; try lia.
-        eapply IHi with (Γ2 := Γ2); eauto.
-        apply G_mono with (S i); eauto; lia.
-      + eapply binding_inv_known_fun; eauto.
-      + eapply binding_inv_exposed_Forall; eauto.
-        eapply set_lists_length_eq; eauto.
-      + apply Included_refl.
-  Qed.
-
-  Lemma fun_known_compat Γ e e' k k' f w xs :
-    K ! f = Some w ->
-    Disjoint _ (FromList xs) (Dom_map K) ->
-
-    trans_correct (FromList xs :|: (f |: Γ)) e e' ->
-    trans_correct (f |: Γ) k k' ->
-    trans_correct Γ (A0.Efun f xs e k) (A1.Efun f w xs e' k').
-  Proof.
-    unfold trans_correct, E, E'.
-    intros HKf HKxs.
-    intros.
-    inv H4.
-    - exists 0, A1.OOT; split; simpl; eauto.
-    - inv H5.
-      edestruct (H0 (i - 1) (M.set f (A0.Vfun f ρ1 xs e) ρ1) (M.set f (Tag w (A1.Vfun f ρ2 xs e')) ρ2)) with (j1 := c) (r1 := r1) as [j2 [r2 [Hk2 Rr]]]; eauto; try lia.
-      + eapply G_subset with (Γ2 := (f |: A1.occurs_free (A1.Efun f w xs e' k'))).
-        eapply G_set; eauto.
-        apply G_mono with i; eauto; lia.
-        * eapply Vfun_V_known; eauto.
-          -- eapply G_wf_env_r; eauto.
-          -- apply G_mono with i; eauto; lia.
-          -- apply A1.free_fun_e_subset.
-        * eapply binding_inv_known_fun; eauto.
-        * apply Included_refl.
-        * apply A1.free_fun_k_subset.
-      + exists (S j2), r2; split; auto.
-        * constructor; simpl; auto.
-          eapply bstep_fuel_exposed_inv; eauto.
-        * apply R_mono with ((i - 1) - c); try lia; auto.
-  Qed.
-
-  Lemma Vfun_V_unknown Γ1 f xs e e' :
-    known_map_inv K ->
-    K ! f = None ->
-    Disjoint _ (FromList xs) (Dom_map K) ->
-    trans_correct (FromList xs :|: (f |: Γ1)) e e' ->
-    forall {i Γ2 ρ1 ρ2},
-      wf_env ρ2 ->
-      G i Γ1 ρ1 Γ2 ρ2 ->
-      A1.occurs_free e' \subset (FromList xs :|: (f |: Γ2)) ->
-      V i (A0.Vfun f ρ1 xs e) (Tag w0 (A1.Vfun f ρ2 xs e')).
-  Proof.
-    unfold trans_correct.
-    intros HK HKf HKxs He i.
-    induction i; simpl; intros; auto;
-      rewrite HKf;
-      repeat (split; auto); intros;
-      try (constructor; apply w0_exposed).
-
-    apply (He (i - (i - j)) ρ3 ρ4); auto.
-    - eapply G_subset with (Γ2 := (FromList xs :|: (f |: Γ2))); eauto.
-      eapply G_set_lists; eauto.
-      eapply G_set; eauto.
-      + apply G_mono with (S i); eauto; lia.
-      + apply V_mono with i; try lia.
-        eapply IHi with (Γ2 := Γ2); eauto.
-        apply G_mono with (S i); eauto; lia.
-      + split; intros; simpl; auto.
-        constructor; apply w0_exposed.
-      + eapply binding_inv_exposed_Forall; eauto.
-        eapply set_lists_length_eq; eauto.
-      + apply Included_refl.
-  Qed.
-
-  Lemma fun_unknown_compat Γ e e' k k' f xs :
-    K ! f = None ->
-    Disjoint _ (FromList xs) (Dom_map K) ->
-
-    trans_correct (FromList xs :|: (f |: Γ)) e e' ->
-    trans_correct (f |: Γ) k k' ->
-    trans_correct Γ (A0.Efun f xs e k) (A1.Efun f w0 xs e' k').
-  Proof.
-    unfold trans_correct, E, E'.
-    intros HKf HKxs.
-    intros.
-    inv H4.
-    - exists 0, A1.OOT; split; simpl; eauto.
-    - inv H5.
-      edestruct (H0 (i - 1) (M.set f (A0.Vfun f ρ1 xs e) ρ1) (M.set f (Tag w0 (A1.Vfun f ρ2 xs e')) ρ2)) with (j1 := c) (r1 := r1) as [j2 [r2 [Hk2 Rr]]]; eauto; try lia.
-      + eapply G_subset with (Γ2 := (f |: A1.occurs_free (A1.Efun f w0 xs e' k'))).
-        eapply G_set; eauto.
-        apply G_mono with i; eauto; lia.
-        * eapply Vfun_V_unknown; eauto.
-          -- eapply G_wf_env_r; eauto.
-          -- apply G_mono with i; eauto; lia.
-          -- apply A1.free_fun_e_subset.
-        * eapply binding_inv_exposed; eauto.
-          constructor; apply w0_exposed.
-        * apply Included_refl.
-        * apply A1.free_fun_k_subset.
-      + exists (S j2), r2; split; auto.
-        * constructor; simpl; auto.
-          eapply bstep_fuel_exposed_inv; eauto.
-        * apply R_mono with ((i - 1) - c); try lia; auto.
-  Qed.
-
-  Lemma app_known_compat Γ xs f w :
-    (K ! f = Some w) ->
-    (~ w \in Exposed) ->
-    Disjoint _ (FromList xs) (Dom_map K) ->
-
-    (f \in Γ) ->
-    (FromList xs \subset Γ) ->
-    trans_correct Γ (A0.Eapp f xs) (A1.Eapp f w xs).
-  Proof.
-    unfold trans_correct, E, E'.
-    intros HKf Hw HKxs.
-    intros; simpl.
-
-    inv H4.
-    - exists 0, A1.OOT; split; simpl; auto.
-    - inv H5.
-      edestruct (G_get H2 f) as [fv2 [Heqfv2 [[Hid HK] HV]]]; eauto.
-      destruct i.
-      inv H3.
-      destruct fv2; simpl in HV;
-        destruct HV as [Hv1 HV];
-        destruct v; try contradiction.
-      specialize (Hid _ HKf).
-      apply same_id_fun in Hid; subst.
-      destruct HV as [Hfeq [Hlen HV]]; subst.
-      destruct (K ! f) eqn:Heqk; try contradiction.
-      + destruct HV as [Heqw [Hex HV]]; subst.
-        inv HKf.
-        clear HK Hex.
-
-        edestruct (G_get_list H2 xs vs) as [vs2 [Heqvs2 [Hexvs Vvs]]]; eauto.
-        eapply A1.free_app_xs_subset; eauto.
-
-        destruct (set_lists_length3 (M.set f (Tag w (A1.Vfun f t l e0)) t) l vs2) as [ρ4 Heqρ4].
-        unfold wval in *.
-        rewrite <- (Forall2_length _ _ _ Vvs).
-        rewrite <- (set_lists_length_eq _ _ _ _ H9); auto.
-
-        assert (HE : E true (i - (i - i)) ρ'' e ρ4 e0).
-        {
-          eapply (HV i vs vs2); eauto.
-          apply V_mono_Forall with (S i); auto; lia.
-        }
-
-        apply (E_mono _ i) in HE; try lia.
-        unfold E in HE.
-        destruct (HE c r1) as [j2 [r2 [He0 Rr]]]; try lia; auto.
-        exists (S j2), r2; split; eauto.
-        constructor; auto.
-        * econstructor; eauto.
-          destruct (exposed_reflect w); try contradiction; auto.
-          -- pose proof He0 as Hr2.
-             apply bstep_fuel_exposed_inv in Hr2.
-             eapply bstep_fuel_exposed; eauto.
-          -- intros; contradiction.
-        * eapply bstep_fuel_exposed_inv; eauto.
-      + destruct HV as [Hex HV].
-        inv Hex.
-        rewrite HKf in Heqk; discriminate.
-  Qed.
-
-  Lemma app_unknown_compat Γ xs f :
-    (K ! f = None) ->
-    Disjoint _ (FromList xs) (Dom_map K) ->
-
-    (f \in Γ) ->
-    (FromList xs \subset Γ) ->
-    trans_correct Γ (A0.Eapp f xs) (A1.Eapp f w0 xs).
-  Proof.
-    unfold trans_correct, E, E'.
-    intros HKf HKxs.
-    intros.
-    inv H4.
-    - exists 0, A1.OOT; split; simpl; auto.
-    - inv H5.
-      edestruct (G_get H2 f) as [fv2 [Heqfv2 [[Hid HK] HV]]]; eauto.
-      destruct i.
-      inv H3.
-      destruct fv2; simpl in HV;
-        destruct HV as [Hv1 HV];
-        destruct v; try contradiction.
-      destruct HV as [Hfeq [Hlen HV]]; subst.
-      rename v into f'.
-      destruct (K ! f') eqn:HeqKf'; try discriminate.
-      + destruct HV as [Heqw [Hex HV]]; subst.
-        specialize (HK HKf).
-        inv HK; contradiction.
-      + destruct HV as [Hex HV].
-        inv Hex.
-        assert (Hw : w = w0) by (apply Exposed_singleton; eauto); subst.
-
-        edestruct (G_get_list H2 xs vs) as [vs2 [Heqvs2 [Hexvs Vvs]]]; eauto.
-        eapply A1.free_app_xs_subset; eauto.
-
-        destruct (set_lists_length3 (M.set f' (Tag w0 (A1.Vfun f' t l e0)) t) l vs2) as [ρ4 Heqρ4].
-        unfold wval in *.
-        rewrite <- (Forall2_length _ _ _ Vvs).
-        rewrite <- (set_lists_length_eq _ _ _ _ H9); auto.
-
-        assert (HE : E true (i - (i - i)) ρ'' e ρ4 e0).
-        {
-          eapply (HV i vs vs2); eauto.
-          apply V_mono_Forall with (S i); auto; lia.
-        }
-
-        apply (E_mono _ i) in HE; try lia.
-        unfold E in HE.
-        destruct (HE c r1) as [j2 [r2 [He0 Rr]]]; try lia; auto.
-        assert (exposed_res r2) by (eapply bstep_fuel_exposed_inv; eauto).
-        exists (S j2), r2; split; eauto; simpl.
-        constructor; auto.
-        econstructor; eauto.
-        destruct (exposed_reflect w0); try contradiction; auto.
-  Qed.
-
-  Lemma letapp_known_compat Γ k k' xs x w f :
-    K ! f = Some w ->
-    (~ w \in Exposed) ->
-    Disjoint _ (FromList xs) (Dom_map K) ->
-    K ! x = None ->
-
-    (f \in Γ) ->
-    (FromList xs \subset Γ) ->
-    trans_correct (x |: Γ) k k' ->
-    trans_correct Γ (A0.Eletapp x f xs k) (A1.Eletapp x f w xs k').
-  Proof.
-    intros HKf Hw HKxs HKx.
-    intros.
-    specialize (app_known_compat Γ xs f w HKf Hw HKxs H H0); intros Ha.
-    unfold trans_correct, E, E' in *.
-    intros.
-
-    assert (HG' : G i Γ ρ1 (occurs_free (A1.Eapp f w xs)) ρ2).
-    {
-      eapply G_subset with (Γ2 := (occurs_free (A1.Eletapp x f w xs k'))); eauto.
-      apply Included_refl.
-      eapply free_app_letapp; eauto.
-    }
-
-    inv H5.
-    - exists 0, OOT; split; simpl; auto.
-    - inv H6.
-      + destruct (Ha i ρ1 ρ2) with (j1 := (S c0)) (r1 := (A0.Res v)) as [j2 [r2 [Hr1 HR]]]; try lia; eauto.
-        * simpl in HR.
-          destruct r2; try contradiction.
-          rename w1 into v0.
-          inv Hr1.
-
-          edestruct (H1 (i - (S c0)) (M.set x v ρ1) (M.set x v0 ρ2)) with (j1 := c') as [j2 [r2 [Hk Rr]]]; eauto; try lia.
-          -- eapply G_subset with (Γ2 := (x |: (A1.occurs_free (A1.Eletapp x f w xs k')))).
-             eapply G_set; eauto.
-             apply G_mono with i; try lia; eauto.
-             eapply binding_inv_exposed; eauto.
-             inv H6; auto.
-             apply Included_refl.
-             apply free_letapp_k_subset.
-          -- exists ((S c) + j2), r2; split.
-             ++ inv H5.
-                rewrite_math ((S c + j2) = S (c + j2)).
-                constructor; auto.
-                ** eapply BStep_letapp_Res; eauto.
-                   intros.
-                   destruct H21; auto.
-                   inv H8.
-                   split; auto.
-                ** eapply bstep_fuel_exposed_inv; eauto.
-             ++ apply R_mono with (i - S c0 - c'); try lia; auto.
-      + eexists; eexists; repeat split; eauto.
-        simpl; auto.
-  Qed.
-
-  Lemma letapp_unknown_compat Γ k k' xs x f :
-    K ! f = None ->
-    Disjoint _ (FromList xs) (Dom_map K) ->
-    K ! x = None ->
-
-    (f \in Γ) ->
-    (FromList xs \subset Γ) ->
-    trans_correct (x |: Γ) k k' ->
-    trans_correct Γ (A0.Eletapp x f xs k) (A1.Eletapp x f w0 xs k').
-  Proof.
-    intros HKf HKxs HKx.
-    intros.
-    specialize (app_unknown_compat Γ xs f HKf HKxs H H0); intros Ha.
-    unfold trans_correct, E, E' in *.
-    intros.
-
-    assert (HG' : G i Γ ρ1 (occurs_free (A1.Eapp f w0 xs)) ρ2).
-    {
-      eapply G_subset with (Γ2 := (occurs_free (A1.Eletapp x f w0 xs k'))); eauto.
-      apply Included_refl.
-      eapply free_app_letapp; eauto.
-    }
-
-    inv H5.
-    - exists 0, OOT; split; simpl; auto.
-    - inv H6.
-      + destruct (Ha i ρ1 ρ2) with (j1 := (S c0)) (r1 := (A0.Res v)) as [j2 [r2 [Hr1 HR]]]; try lia; eauto.
-        * simpl in HR.
-          destruct r2; try contradiction.
-          rename w into v0.
-          inv Hr1.
-
-          edestruct (H1 (i - (S c0)) (M.set x v ρ1) (M.set x v0 ρ2)) with (j1 := c') as [j2 [r2 [Hk Rr]]]; eauto; try lia.
-          -- eapply G_subset with (Γ2 := (x |: (A1.occurs_free (A1.Eletapp x f w0 xs k')))).
-             eapply G_set; eauto.
-             apply G_mono with i; try lia; eauto.
-             eapply binding_inv_exposed; eauto.
-             inv H6; auto.
-             apply Included_refl.
-             apply free_letapp_k_subset.
-          -- exists ((S c) + j2), r2; split.
-             ++ inv H5.
-                rewrite_math ((S c + j2) = S (c + j2)).
-                constructor; auto.
-                ** eapply BStep_letapp_Res; eauto.
-                   intros.
-                   destruct H21; auto.
-                   inv H8.
-                   split; auto.
-                ** eapply bstep_fuel_exposed_inv; eauto.
-             ++ apply R_mono with (i - S c0 - c'); try lia; auto.
-      + eexists; eexists; repeat split; eauto.
-        simpl; auto.
-  Qed.
-
-  Lemma constr_compat Γ x t xs k k' :
-    K ! x = None ->
-    Disjoint _ (FromList xs) (Dom_map K) ->
-
-    (FromList xs \subset Γ) ->
-    trans_correct (x |: Γ) k k' ->
-    trans_correct Γ (A0.Econstr x t xs k) (A1.Econstr x w0 t xs k').
-  Proof.
-    unfold trans_correct, E, E'.
-    intros.
-    inv H6.
-    - exists 0, A1.OOT; split; simpl; auto.
-    - inv H7.
-      destruct (G_get_list H4 xs vs) as [vs' [Heqvs' Hvs]]; auto.
-      + eapply A1.free_constr_xs_subset; eauto.
-      + inv Hvs.
-        assert (wf_val (Tag w0 (A1.Vconstr t vs'))).
-        {
-          apply wf_val_Vconstr; auto.
-          eapply V_wf_val_Forall_r; eauto.
-        }
-
-        assert (exposed (Tag w0 (A1.Vconstr t vs'))).
-        {
-          constructor; auto.
-          apply w0_exposed.
-        }
-
-        assert (length vs = length vs').
-        {
-          unfold wval in *.
-          rewrite <- (get_list_length_eq _ _ _ H13).
-          rewrite <- (get_list_length_eq _ _ _ Heqvs'); auto.
-        }
-
-        edestruct (H2 i (M.set x (A0.Vconstr t vs) ρ1) (M.set x (Tag w0 (A1.Vconstr t vs')) ρ2)) with (j1 := c) (r1 := r1) as [j2 [r2 [Hk' Rr]]]; eauto; try lia.
-        * eapply G_subset with (Γ2 := (x |: (A1.occurs_free (A1.Econstr x w0 t xs k')))).
+      trans_correct (x |: Γ) e e' ->
+      trans_correct Γ (A0.Eproj x i y e) (A1.Eproj x w0 i y e').
+    Proof.
+      unfold trans_correct, E, E'.
+      intros.
+      inv H6.
+      - exists 0, A1.OOT; split; simpl; auto.
+      - inv H7.
+        edestruct (G_get H4 y) as [v2 [Heqv2 HV]]; eauto.
+        destruct i0.
+        inv H5.
+        destruct v2;
+          simpl in HV;
+          destruct HV as [Hb [Hv HV]]; subst;
+          destruct v0; try contradiction.
+        rename l into vs'.
+        rename c0 into t'.
+        destruct HV as [Hex [Heqt HFvs]]; subst.
+        destruct (Forall2_nth_error H14 HFvs) as [v' [Heqv' HFv]].
+        edestruct (H2 i0 (M.set x v ρ1) (M.set x v' ρ2)) with (j1 := c) as [j2 [r2 [He' HR]]]; eauto; try lia.
+        + eapply G_subset with (Γ2 := (x |: (A1.occurs_free (A1.Eproj x w0 i y e')))).
           eapply G_set; eauto.
-          -- destruct i; simpl; repeat (split; eauto).
-             eapply V_mono_Forall; eauto; lia.
-          -- eapply binding_inv_exposed; eauto.
-          -- apply Included_refl.
-          -- apply A1.free_constr_k_subset.
-        * exists (S j2), r2; split; eauto.
-          -- econstructor.
-             econstructor; eauto.
-             eapply bstep_fuel_exposed_inv in Hk'; eauto.
-          -- apply R_mono with (i - c); try lia; auto.
-  Qed.
+          eapply G_mono with (S i0); eauto; try lia.
+          eapply binding_inv_exposed; eauto.
+          eapply Forall_nth_error; eauto.
+          inv Hex; auto.
+          apply Included_refl.
+          apply A1.free_proj_k_subset.
+        + assert (Hw : w = w0).
+          {
+            inv Hex.
+            apply Exposed_singleton; eauto.
+          }
+          subst.
 
-  Lemma proj_compat Γ x i y e e' :
-    K ! x = None ->
-    K ! y = None ->
+          exists (S j2), r2; split; eauto.
+          constructor.
+          econstructor; eauto.
+          eapply bstep_fuel_exposed_inv; eauto.
+    Qed.
 
-    (y \in Γ) ->
-    trans_correct (x |: Γ) e e' ->
-    trans_correct Γ (A0.Eproj x i y e) (A1.Eproj x w0 i y e').
-  Proof.
-    unfold trans_correct, E, E'.
-    intros.
-    inv H6.
-    - exists 0, A1.OOT; split; simpl; auto.
-    - inv H7.
-      edestruct (G_get H4 y) as [v2 [Heqv2 HV]]; eauto.
-      destruct i0.
-      inv H5.
-      destruct v2;
-        simpl in HV;
-        destruct HV as [Hb [Hv HV]]; subst;
-        destruct v0; try contradiction.
-      rename l into vs'.
-      rename c0 into t'.
-      destruct HV as [Hex [Heqt HFvs]]; subst.
-      destruct (Forall2_nth_error H14 HFvs) as [v' [Heqv' HFv]].
-      edestruct (H2 i0 (M.set x v ρ1) (M.set x v' ρ2)) with (j1 := c) as [j2 [r2 [He' HR]]]; eauto; try lia.
-      + eapply G_subset with (Γ2 := (x |: (A1.occurs_free (A1.Eproj x w0 i y e')))).
-        eapply G_set; eauto.
-        eapply G_mono with (S i0); eauto; try lia.
-        eapply binding_inv_exposed; eauto.
-        eapply Forall_nth_error; eauto.
-        inv Hex; auto.
-        apply Included_refl.
-        apply A1.free_proj_k_subset.
-      + assert (Hw : w = w0).
+    Lemma case_nil_compat Γ x:
+      K ! x = None ->
+      (x \in Γ) ->
+      trans_correct Γ (A0.Ecase x []) (A1.Ecase x w0 []).
+    Proof.
+      unfold trans_correct, E, E'.
+      intros.
+      inv H4.
+      - exists 0, A1.OOT; split; simpl; auto.
+      - inv H5.
+        inv H8.
+    Qed.
+
+    Lemma case_cons_compat Γ x t e e' cl cl':
+      K ! x = None ->
+      (x \in Γ) ->
+      trans_correct Γ e e' ->
+      trans_correct Γ (A0.Ecase x cl) (A1.Ecase x w0 cl') ->
+      trans_correct Γ (A0.Ecase x ((t, e) :: cl)) (A1.Ecase x w0 ((t, e') :: cl')).
+    Proof.
+      unfold trans_correct, E, E'.
+      intros.
+      inv H6.
+      - exists 0, OOT; split; simpl; eauto.
+      - inv H7.
+        edestruct (G_get H4) as [v2 [Heqv2 HV]]; eauto.
+        destruct v2.
+        destruct i.
+        inv H5.
+        destruct v; simpl in HV;
+          destruct HV as [Hb [Hv2 HV]]; subst;
+          subst; try contradiction.
+        destruct HV as [Hex [Heqt HFvs]]; subst.
+        assert (Hw : w = w0).
         {
           inv Hex.
           apply Exposed_singleton; eauto.
         }
         subst.
 
-        exists (S j2), r2; split; eauto.
-        constructor.
-        econstructor; eauto.
-        eapply bstep_fuel_exposed_inv; eauto.
-  Qed.
+        inv H10.
+        + edestruct (H1 i ρ1 ρ2) with (j1 := c) as [j2 [r2 [He' HR]]]; eauto; try lia.
+          eapply G_subset with (Γ2 := (A1.occurs_free (A1.Ecase x w0 ((c0, e') :: cl')))); eauto.
+          eapply G_mono; eauto.
+          apply Included_refl.
+          apply A1.free_case_hd_subset.
 
-  Lemma case_nil_compat Γ x:
-    K ! x = None ->
-    (x \in Γ) ->
-    trans_correct Γ (A0.Ecase x []) (A1.Ecase x w0 []).
-  Proof.
-    unfold trans_correct, E, E'.
-    intros.
-    inv H4.
-    - exists 0, A1.OOT; split; simpl; auto.
-    - inv H5.
-      inv H8.
-  Qed.
+          exists (S j2), r2; split; eauto.
+          econstructor; eauto.
+          eapply bstep_fuel_exposed_inv; eauto.
+        + edestruct (H2 (S i) ρ1 ρ2) with (j1 := S c) (r1 := r1) as [j2 [r2 [He' HR]]]; eauto; try lia.
+          eapply G_subset; eauto.
+          apply Included_refl.
+          apply A1.free_case_tl_subset; auto.
 
-  Lemma case_cons_compat Γ x t e e' cl cl':
-    K ! x = None ->
-    (x \in Γ) ->
-    trans_correct Γ e e' ->
-    trans_correct Γ (A0.Ecase x cl) (A1.Ecase x w0 cl') ->
-    trans_correct Γ (A0.Ecase x ((t, e) :: cl)) (A1.Ecase x w0 ((t, e') :: cl')).
-  Proof.
-    unfold trans_correct, E, E'.
-    intros.
-    inv H6.
-    - exists 0, OOT; split; simpl; eauto.
-    - inv H7.
-      edestruct (G_get H4) as [v2 [Heqv2 HV]]; eauto.
-      destruct v2.
-      destruct i.
-      inv H5.
-      destruct v; simpl in HV;
-        destruct HV as [Hb [Hv2 HV]]; subst;
-        subst; try contradiction.
-      destruct HV as [Hex [Heqt HFvs]]; subst.
-      assert (Hw : w = w0).
-      {
-        inv Hex.
-        apply Exposed_singleton; eauto.
-      }
-      subst.
+          exists j2, r2; split; eauto.
+          inv He'; auto.
+          inv H6.
+          rewrite Heqv2 in H12; inv H12; eauto.
+    Qed.
 
-      inv H10.
-      + edestruct (H1 i ρ1 ρ2) with (j1 := c) as [j2 [r2 [He' HR]]]; eauto; try lia.
-        eapply G_subset with (Γ2 := (A1.occurs_free (A1.Ecase x w0 ((c0, e') :: cl')))); eauto.
-        eapply G_mono; eauto.
-        apply Included_refl.
-        apply A1.free_case_hd_subset.
+    (* Fundamental Property *)
+    Lemma fundamental_property {Γ e e'}:
+      trans Γ e e' -> trans_correct Γ e e'.
+    Proof.
+      intros.
+      induction H; intros.
+      - eapply ret_compat; eauto.
+      - eapply fun_known_compat; eauto.
+      - eapply fun_unknown_compat; eauto.
+      - eapply app_known_compat; eauto.
+      - eapply app_unknown_compat; eauto.
+      - eapply letapp_known_compat; eauto.
+      - eapply letapp_unknown_compat; eauto.
+      - eapply constr_compat; eauto.
+      - eapply proj_compat; eauto.
+      - eapply case_nil_compat; eauto.
+      - eapply case_cons_compat; eauto.
+    Qed.
 
-        exists (S j2), r2; split; eauto.
-        econstructor; eauto.
-        eapply bstep_fuel_exposed_inv; eauto.
-      + edestruct (H2 (S i) ρ1 ρ2) with (j1 := S c) (r1 := r1) as [j2 [r2 [He' HR]]]; eauto; try lia.
-        eapply G_subset; eauto.
-        apply Included_refl.
-        apply A1.free_case_tl_subset; auto.
+    (* Top Level *)
+    Definition binding_inv_top x v :=
+      K ! x = None /\ exposed v.
 
-        exists j2, r2; split; eauto.
-        inv He'; auto.
-        inv H6.
-        rewrite Heqv2 in H12; inv H12; eauto.
-  Qed.
+    Lemma binding_inv_top_exposed x v :
+      K ! x = None ->
+      exposed v ->
+      binding_inv_top x v.
+    Proof. intros. repeat (split; auto). Qed.
 
-  (* Fundamental Property *)
-  Lemma fundamental_property {Γ e e'}:
-    trans Γ e e' -> trans_correct Γ e e'.
-  Proof.
-    intros.
-    induction H; intros.
-    - eapply ret_compat; eauto.
-    - eapply fun_known_compat; eauto.
-    - eapply fun_unknown_compat; eauto.
-    - eapply app_known_compat; eauto.
-    - eapply app_unknown_compat; eauto.
-    - eapply letapp_known_compat; eauto.
-    - eapply letapp_unknown_compat; eauto.
-    - eapply constr_compat; eauto.
-    - eapply proj_compat; eauto.
-    - eapply case_nil_compat; eauto.
-    - eapply case_cons_compat; eauto.
-  Qed.
+    Lemma binding_inv_top_exposed_Forall xs :
+      forall vs,
+        Disjoint _ (FromList xs) (Dom_map K) ->
+        length xs = length vs ->
+        Forall exposed vs ->
+        Forall2 binding_inv_top xs vs.
+    Proof.
+      induction xs; simpl; intros;
+        destruct vs; try discriminate; auto.
+      inv H0; inv H1.
+      apply Disjoint_FromList_cons_inv in H.
+      inv H.
+      constructor; auto.
+      apply binding_inv_top_exposed; auto.
+    Qed.
 
-  (* Top Level *)
-  Definition binding_inv_top x v :=
-    K ! x = None /\ exposed v.
+    Lemma binding_inv_top_binding_inv x v :
+      binding_inv_top x v ->
+      binding_inv x v.
+    Proof.
+      unfold binding_inv_top.
+      intro H; inv H.
+      eapply binding_inv_exposed; eauto.
+    Qed.
 
-  Lemma binding_inv_top_exposed x v :
-    K ! x = None ->
-    exposed v ->
-    binding_inv_top x v.
-  Proof. intros. repeat (split; auto). Qed.
+    Definition G_top i Γ1 ρ1 Γ2 ρ2 :=
+      wf_env ρ2 /\
+      Γ2 \subset Γ1 /\
+      forall x,
+        (x \in Γ1) ->
+        exists v1 v2,
+          M.get x ρ1 = Some v1 /\
+          M.get x ρ2 = Some v2 /\
+          binding_inv_top x v2 /\
+          V i v1 v2.
 
-  Lemma binding_inv_top_exposed_Forall xs :
-    forall vs,
-      Disjoint _ (FromList xs) (Dom_map K) ->
-      length xs = length vs ->
-      Forall exposed vs ->
-      Forall2 binding_inv_top xs vs.
-  Proof.
-    induction xs; simpl; intros;
-      destruct vs; try discriminate; auto.
-    inv H0; inv H1.
-    apply Disjoint_FromList_cons_inv in H.
-    inv H.
-    constructor; auto.
-    apply binding_inv_top_exposed; auto.
-  Qed.
-
-  Lemma binding_inv_top_binding_inv x v :
-    binding_inv_top x v ->
-    binding_inv x v.
-  Proof.
-    unfold binding_inv_top.
-    intro H; inv H.
-    eapply binding_inv_exposed; eauto.
-  Qed.
-
-  Definition G_top i Γ1 ρ1 Γ2 ρ2 :=
-    wf_env ρ2 /\
-    Γ2 \subset Γ1 /\
-    forall x,
-      (x \in Γ1) ->
-      exists v1 v2,
-        M.get x ρ1 = Some v1 /\
-        M.get x ρ2 = Some v2 /\
-        binding_inv_top x v2 /\
-        V i v1 v2.
-
-  Lemma G_top_wf_env_r i Γ1 ρ1 Γ2 ρ2 :
-    G_top i Γ1 ρ1 Γ2 ρ2 ->
-    wf_env ρ2.
-  Proof. unfold G_top. intros; tauto. Qed.
-
-  Lemma G_top_subset_inv i Γ1 ρ1 Γ2 ρ2 :
-    G_top i Γ1 ρ1 Γ2 ρ2 ->
-    Γ2 \subset Γ1.
-  Proof. unfold G_top; intros; tauto. Qed.
-
-  Lemma G_top_subset i Γ1 ρ1 Γ2 ρ2 Γ3 Γ4 :
-    G_top i Γ1 ρ1 Γ2 ρ2 ->
-    Γ3 \subset Γ1 ->
-    Γ4 \subset Γ3 ->
-    G_top i Γ3 ρ1 Γ4 ρ2.
-  Proof.
-    unfold G_top.
-    intros.
-    destruct H as [Hr [Hs HG]].
-    repeat (split; auto).
-  Qed.
-
-  Lemma G_top_G : forall {i Γ1 ρ1 Γ2 ρ2},
+    Lemma G_top_wf_env_r i Γ1 ρ1 Γ2 ρ2 :
       G_top i Γ1 ρ1 Γ2 ρ2 ->
-      G i Γ1 ρ1 Γ2 ρ2.
-  Proof.
-    unfold G_top, G.
-    intros.
-    destruct H as [HΓ [Hρ HG]].
-    unfold Ensembles.Included, Ensembles.In, Dom_map in *.
-    split; auto; intros.
-    edestruct HG as [v1' [v2 [Heqv1 [Heqv2 [[HKx Hex] HV]]]]]; eauto.
-    rewrite Heqv1 in H0; inv H0; eauto.
-    eexists; split; eauto.
-    split; auto.
-    eapply binding_inv_exposed; eauto.
-  Qed.
+      wf_env ρ2.
+    Proof. unfold G_top. intros; tauto. Qed.
 
-  Lemma G_G_top i Γ1 ρ1 Γ2 ρ2 :
-    G i Γ1 ρ1 Γ2 ρ2 ->
-    Γ2 \subset Γ1 ->
-    G_top i Γ1 ρ1 Γ2 ρ2.
-  Proof.
-    unfold G, G_top.
-    intros.
-    destruct H as [Hρ HG].
-    repeat (split; auto); intros.
-  Abort.
+    Lemma G_top_subset_inv i Γ1 ρ1 Γ2 ρ2 :
+      G_top i Γ1 ρ1 Γ2 ρ2 ->
+      Γ2 \subset Γ1.
+    Proof. unfold G_top; intros; tauto. Qed.
 
-  Definition trans_correct_top etop etop' :=
-    A1.occurs_free etop' \subset A0.occurs_free etop /\
-    forall i ρ1 ρ2,
+    Lemma G_top_subset i Γ1 ρ1 Γ2 ρ2 Γ3 Γ4 :
+      G_top i Γ1 ρ1 Γ2 ρ2 ->
+      Γ3 \subset Γ1 ->
+      Γ4 \subset Γ3 ->
+      G_top i Γ3 ρ1 Γ4 ρ2.
+    Proof.
+      unfold G_top.
+      intros.
+      destruct H as [Hr [Hs HG]].
+      repeat (split; auto).
+    Qed.
+
+    Lemma G_top_G : forall {i Γ1 ρ1 Γ2 ρ2},
+        G_top i Γ1 ρ1 Γ2 ρ2 ->
+        G i Γ1 ρ1 Γ2 ρ2.
+    Proof.
+      unfold G_top, G.
+      intros.
+      destruct H as [HΓ [Hρ HG]].
+      unfold Ensembles.Included, Ensembles.In, Dom_map in *.
+      split; auto; intros.
+      edestruct HG as [v1' [v2 [Heqv1 [Heqv2 [[HKx Hex] HV]]]]]; eauto.
+      rewrite Heqv1 in H0; inv H0; eauto.
+      eexists; split; eauto.
+      split; auto.
+      eapply binding_inv_exposed; eauto.
+    Qed.
+
+    Lemma G_G_top i Γ1 ρ1 Γ2 ρ2 :
+      G i Γ1 ρ1 Γ2 ρ2 ->
+      Γ2 \subset Γ1 ->
+      G_top i Γ1 ρ1 Γ2 ρ2.
+    Proof.
+      unfold G, G_top.
+      intros.
+      destruct H as [Hρ HG].
+      repeat (split; auto); intros.
+    Abort.
+
+    Definition trans_correct_top etop etop' :=
+      A1.occurs_free etop' \subset A0.occurs_free etop /\
+        forall i ρ1 ρ2,
+          known_map_inv K ->
+          G_top i (A0.occurs_free etop) ρ1 (A1.occurs_free etop') ρ2 ->
+          E true i ρ1 etop ρ2 etop'.
+
+    Lemma trans_correct_top_subset e1 e2 :
+      trans_correct_top e1 e2 ->
+      A1.occurs_free e2 \subset A0.occurs_free e1.
+    Proof.
+      unfold trans_correct_top.
+      intros.
+      inv H; auto.
+    Qed.
+
+    Lemma trans_correct_subset Γ1 Γ2 e1 e2 :
+      trans_correct Γ1 e1 e2 ->
+      Γ1 \subset Γ2 ->
+      trans_correct Γ2 e1 e2.
+    Proof.
+      unfold trans_correct.
+      intros.
+      eapply H; eauto.
+      eapply G_subset; eauto.
+      apply Included_refl.
+    Qed.
+
+    Lemma trans_correct_top_trans_correct e1 e2 :
+      trans_correct_top e1 e2 ->
+      trans_correct (A0.occurs_free e1) e1 e2.
+    Proof.
+      unfold trans_correct_top, trans_correct.
+      intros.
+      destruct H as [HS H].
+      eapply H; eauto.
+      (* eapply G_G_top; eauto. *)
+    Abort.
+
+    (* [trans_correct] is stronger than [trans_correct_top] due to [G_top] *)
+    Lemma trans_correct_trans_correct_top e1 e2 :
+      A1.occurs_free e2 \subset A0.occurs_free e1 ->
+      trans_correct (A0.occurs_free e1) e1 e2 ->
+      trans_correct_top e1 e2.
+    Proof.
+      unfold trans_correct_top, trans_correct.
+      intros.
+      split; auto; intros.
+      eapply H0; eauto.
+      eapply G_top_G; eauto.
+    Qed.
+
+    Theorem top etop etop':
+      trans (A0.occurs_free etop) etop etop' ->
+      trans_correct_top etop etop'.
+    Proof.
+      intros H.
+      specialize (fundamental_property H).
+      eapply trans_correct_trans_correct_top; eauto.
+      eapply trans_exp_inv; eauto.
+    Qed.
+
+    (* Cross-language Compositionality *)
+
+    (* Adequacy *)
+    Theorem adequacy e1 e2:
       known_map_inv K ->
-      G_top i (A0.occurs_free etop) ρ1 (A1.occurs_free etop') ρ2 ->
-      E true i ρ1 etop ρ2 etop'.
+      trans_correct_top e1 e2 ->
+      forall ρ1 ρ2,
+        wf_env ρ2 ->
+        (forall k, G_top k (A0.occurs_free e1) ρ1 (A1.occurs_free e2) ρ2) ->
+        forall j1 r1,
+          A0.bstep_fuel ρ1 e1 j1 r1 ->
+          exists j2 r2,
+            A1.bstep_fuel true ρ2 e2 j2 r2 /\
+            (forall k, R k r1 r2).
+    Proof.
+      intros HK; intros.
+      unfold trans_correct_top in H.
+      destruct H as [HS HT].
 
-  Lemma trans_correct_top_subset e1 e2 :
-    trans_correct_top e1 e2 ->
-    A1.occurs_free e2 \subset A0.occurs_free e1.
-  Proof.
-    unfold trans_correct_top.
-    intros.
-    inv H; auto.
-  Qed.
+      assert (HE : E true j1 ρ1 e1 ρ2 e2) by (eapply (HT j1); eauto).
+      edestruct (HE j1) as [j2 [r2 [Hstep2 HR]]]; eauto.
+      eexists; eexists; split; eauto.
 
-  Lemma trans_correct_subset Γ1 Γ2 e1 e2 :
-    trans_correct Γ1 e1 e2 ->
-    Γ1 \subset Γ2 ->
-    trans_correct Γ2 e1 e2.
-  Proof.
-    unfold trans_correct.
-    intros.
-    eapply H; eauto.
-    eapply G_subset; eauto.
-    apply Included_refl.
-  Qed.
+      intros.
+      assert (HE' : E true (j1 + k) ρ1 e1 ρ2 e2) by (eapply HT; eauto).
+      edestruct (HE' j1) as [j2' [r2' [Hstep2' HR']]]; eauto; try lia.
 
-  Lemma trans_correct_top_trans_correct e1 e2 :
-    trans_correct_top e1 e2 ->
-    trans_correct (A0.occurs_free e1) e1 e2.
-  Proof.
-    unfold trans_correct_top, trans_correct.
-    intros.
-    destruct H as [HS H].
-    eapply H; eauto.
-    (* eapply G_G_top; eauto. *)
-  Abort.
+      rewrite_math (j1 + k - j1 = k).
+      rewrite_math (j1 - j1 = 0).
 
-  (* [trans_correct] is stronger than [trans_correct_top] due to [G_top] *)
-  Lemma trans_correct_trans_correct_top e1 e2 :
-    A1.occurs_free e2 \subset A0.occurs_free e1 ->
-    trans_correct (A0.occurs_free e1) e1 e2 ->
-    trans_correct_top e1 e2.
-  Proof.
-    unfold trans_correct_top, trans_correct.
-    intros.
-    split; auto; intros.
-    eapply H0; eauto.
-    eapply G_top_G; eauto.
-  Qed.
+      destruct r2; destruct r2'; destruct r1;
+        simpl in *; auto; try contradiction.
 
-  Theorem top etop etop':
-    trans (A0.occurs_free etop) etop etop' ->
-    trans_correct_top etop etop'.
-  Proof.
-    intros H.
-    specialize (fundamental_property H).
-    eapply trans_correct_trans_correct_top; eauto.
-    eapply trans_exp_inv; eauto.
-  Qed.
+      edestruct (A1.bstep_fuel_deterministic w w1 Hstep2 Hstep2'); subst; eauto.
+    Qed.
 
-  (* Cross-language Compositionality *)
+    (* Behavioral Refinement *)
+    Inductive val_ref_ : A0.val -> A1.wval -> Prop :=
+    | Ref_Vfun :
+      forall f1 ρ1 w xs1 e1 f2 ρ2 xs2 e2,
+        val_ref_ (A0.Vfun f1 ρ1 xs1 e1) (Tag w (A1.Vfun f2 ρ2 xs2 e2))
 
-  (* Adequacy *)
-  Theorem adequacy e1 e2:
-    known_map_inv K ->
-    trans_correct_top e1 e2 ->
-    forall ρ1 ρ2,
-      wf_env ρ2 ->
-      (forall k, G_top k (A0.occurs_free e1) ρ1 (A1.occurs_free e2) ρ2) ->
-      forall j1 r1,
-        A0.bstep_fuel ρ1 e1 j1 r1 ->
-        exists j2 r2,
-          A1.bstep_fuel true ρ2 e2 j2 r2 /\
-          (forall k, R k r1 r2).
-  Proof.
-    intros HK; intros.
-    unfold trans_correct_top in H.
-    destruct H as [HS HT].
+    | Ref_Vconstr_nil :
+      forall c,
+        val_ref_ (A0.Vconstr c []) (Tag w0 (A1.Vconstr c []))
 
-    assert (HE : E true j1 ρ1 e1 ρ2 e2) by (eapply (HT j1); eauto).
-    edestruct (HE j1) as [j2 [r2 [Hstep2 HR]]]; eauto.
-    eexists; eexists; split; eauto.
+    | Ref_Vconstr_cons :
+      forall c v1 v2 vs1 vs2,
+        val_ref_ v1 v2 ->
+        val_ref_ (A0.Vconstr c vs1) (Tag w0 (A1.Vconstr c vs2)) ->
+        val_ref_ (A0.Vconstr c (v1 :: vs1)) (Tag w0 (A1.Vconstr c (v2 :: vs2))).
 
-    intros.
-    assert (HE' : E true (j1 + k) ρ1 e1 ρ2 e2) by (eapply HT; eauto).
-    edestruct (HE' j1) as [j2' [r2' [Hstep2' HR']]]; eauto; try lia.
+    Hint Constructors val_ref_ : core.
 
-    rewrite_math (j1 + k - j1 = k).
-    rewrite_math (j1 - j1 = 0).
+    Definition val_ref := val_ref_.
 
-    destruct r2; destruct r2'; destruct r1;
-      simpl in *; auto; try contradiction.
+    Hint Unfold val_ref : core.
 
-    edestruct (A1.bstep_fuel_deterministic w w1 Hstep2 Hstep2'); subst; eauto.
-  Qed.
+    Lemma val_ref_Vconstr c vs1 vs2 :
+      Forall2 val_ref vs1 vs2 ->
+      val_ref (A0.Vconstr c vs1) (Tag w0 (A1.Vconstr c vs2)).
+    Proof.
+      intros.
+      induction H; simpl; auto.
+    Qed.
 
-  (* Behavioral Refinement *)
-  Inductive val_ref_ : A0.val -> A1.wval -> Prop :=
-  | Ref_Vfun :
-    forall f1 ρ1 w xs1 e1 f2 ρ2 xs2 e2,
-      val_ref_ (A0.Vfun f1 ρ1 xs1 e1) (Tag w (A1.Vfun f2 ρ2 xs2 e2))
+    Theorem V_val_ref {v1 v2} :
+      (forall i, V i v1 v2) ->
+      val_ref v1 v2.
+    Proof.
+      unfold val_ref.
+      revert v2.
+      induction v1 using val_ind'; intros; simpl.
+      - specialize (H 0).
+        destruct v2.
+        simpl in H.
+        destruct H as [Hw HV].
+        destruct v; try contradiction.
+        destruct HV as [Hex [Hc Hlen]]; subst.
+        destruct l; try discriminate.
+        inv Hex.
+        apply Exposed_singleton in H1; subst; auto.
+      - destruct v2.
+        pose proof (H 0) as H0; simpl in *.
+        destruct H0 as [Hw HV].
+        destruct v; try contradiction.
+        destruct HV as [Hex [Hc Hlen]]; subst.
 
-  | Ref_Vconstr_nil :
-    forall c,
-      val_ref_ (A0.Vconstr c []) (Tag w0 (A1.Vconstr c []))
+        destruct l0; simpl in *; inv Hlen.
+        inv Hex.
+        apply Exposed_singleton in H3; subst.
 
-  | Ref_Vconstr_cons :
-    forall c v1 v2 vs1 vs2,
-      val_ref_ v1 v2 ->
-      val_ref_ (A0.Vconstr c vs1) (Tag w0 (A1.Vconstr c vs2)) ->
-      val_ref_ (A0.Vconstr c (v1 :: vs1)) (Tag w0 (A1.Vconstr c (v2 :: vs2))).
-
-  Hint Constructors val_ref_ : core.
-
-  Definition val_ref := val_ref_.
-
-  Hint Unfold val_ref : core.
-
-  Lemma val_ref_Vconstr c vs1 vs2 :
-    Forall2 val_ref vs1 vs2 ->
-    val_ref (A0.Vconstr c vs1) (Tag w0 (A1.Vconstr c vs2)).
-  Proof.
-    intros.
-    induction H; simpl; auto.
-  Qed.
-
-  Theorem V_val_ref {v1 v2} :
-    (forall i, V i v1 v2) ->
-    val_ref v1 v2.
-  Proof.
-    unfold val_ref.
-    revert v2.
-    induction v1 using val_ind'; intros; simpl.
-    - specialize (H 0).
-      destruct v2.
-      simpl in H.
-      destruct H as [Hw HV].
-      destruct v; try contradiction.
-      destruct HV as [Hex [Hc Hlen]]; subst.
-      destruct l; try discriminate.
-      inv Hex.
-      apply Exposed_singleton in H1; subst; auto.
-    - destruct v2.
-      pose proof (H 0) as H0; simpl in *.
-      destruct H0 as [Hw HV].
-      destruct v; try contradiction.
-      destruct HV as [Hex [Hc Hlen]]; subst.
-
-      destruct l0; simpl in *; inv Hlen.
-      inv Hex.
-      apply Exposed_singleton in H3; subst.
-
-      assert (HV' : forall i, V i v1 t /\ V i (A0.Vconstr c l) (Tag w0 (A1.Vconstr c l0))).
-      {
-        intros.
-        specialize (H (S i)); simpl in *.
-        destruct H as [_ [He [Hc HFV]]]; subst.
-        inv HFV.
-        split; auto.
-
-        assert (He' : exposed (Tag w0 (A1.Vconstr c l0))) by (inv He; inv H5; auto).
-
-        assert (Hw' : wf_val (Tag w0 (A1.Vconstr c l0))).
+        assert (HV' : forall i, V i v1 t /\ V i (A0.Vconstr c l) (Tag w0 (A1.Vconstr c l0))).
         {
-          constructor; intros; auto.
-          inv Hw.
-          inv H4; auto.
+          intros.
+          specialize (H (S i)); simpl in *.
+          destruct H as [_ [He [Hc HFV]]]; subst.
+          inv HFV.
+          split; auto.
+
+          assert (He' : exposed (Tag w0 (A1.Vconstr c l0))) by (inv He; inv H5; auto).
+
+          assert (Hw' : wf_val (Tag w0 (A1.Vconstr c l0))).
+          {
+            constructor; intros; auto.
+            inv Hw.
+            inv H4; auto.
+          }
+
+          destruct i; simpl in *;
+            repeat (split; auto);
+            try (eapply V_mono_Forall with (S i); eauto).
         }
 
-        destruct i; simpl in *;
-          repeat (split; auto);
-          try (eapply V_mono_Forall with (S i); eauto).
-      }
+        assert (HV0 : forall i, V i v1 t) by (intros; destruct (HV' i); auto).
+        assert (HV1 : forall i, V i (A0.Vconstr c l) (Tag w0 (A1.Vconstr c l0))) by (intros; destruct (HV' i); auto).
 
-      assert (HV0 : forall i, V i v1 t) by (intros; destruct (HV' i); auto).
-      assert (HV1 : forall i, V i (A0.Vconstr c l) (Tag w0 (A1.Vconstr c l0))) by (intros; destruct (HV' i); auto).
+        auto.
+      - specialize (H 0); simpl in *.
+        destruct H as [Hw HV].
+        destruct v2; try contradiction; auto.
+        destruct v; try contradiction; auto.
+    Qed.
 
-      auto.
-    - specialize (H 0); simpl in *.
-      destruct H as [Hw HV].
-      destruct v2; try contradiction; auto.
-      destruct v; try contradiction; auto.
-  Qed.
+    Corollary R_res_val_ref {v1 v2} :
+      (forall i, R i (A0.Res v1) (A1.Res v2)) ->
+      val_ref v1 v2.
+    Proof.
+      intros; eapply V_val_ref; eauto.
+    Qed.
 
-  Corollary R_res_val_ref {v1 v2} :
-    (forall i, R i (A0.Res v1) (A1.Res v2)) ->
-    val_ref v1 v2.
-  Proof.
-    intros; eapply V_val_ref; eauto.
-  Qed.
+    (* Linking Compat Lemmas *)
 
-  (* Linking Compat Lemmas *)
+    (* Top-level Environment Lemmas *)
+    Lemma G_top_get {Γ1 Γ2 i ρ1 ρ2}:
+      G_top i Γ1 ρ1 Γ2 ρ2 ->
+      forall x,
+        (x \in Γ1) ->
+        exists v1 v2,
+          M.get x ρ1 = Some v1 /\
+          M.get x ρ2 = Some v2 /\
+          binding_inv_top x v2 /\
+          V i v1 v2.
+    Proof.
+      unfold G.
+      intros.
+      destruct H as [Hr1 [HΓ HG]].
+      eapply (HG x); eauto.
+    Qed.
 
-  (* Top-level Environment Lemmas *)
-  Lemma G_top_get {Γ1 Γ2 i ρ1 ρ2}:
-    G_top i Γ1 ρ1 Γ2 ρ2 ->
-    forall x,
-      (x \in Γ1) ->
-      exists v1 v2,
-        M.get x ρ1 = Some v1 /\
-        M.get x ρ2 = Some v2 /\
-        binding_inv_top x v2 /\
-        V i v1 v2.
-  Proof.
-    unfold G.
-    intros.
-    destruct H as [Hr1 [HΓ HG]].
-    eapply (HG x); eauto.
-  Qed.
+    Lemma G_top_get_list {i Γ1 ρ1 Γ2 ρ2} :
+      G_top i Γ1 ρ1 Γ2 ρ2 ->
+      forall xs,
+        (FromList xs) \subset Γ1 ->
+        Disjoint _ (FromList xs) (Dom_map K) ->
+        exists vs1 vs2,
+          get_list xs ρ1 = Some vs1 /\
+          get_list xs ρ2 = Some vs2 /\
+          Forall exposed vs2 /\
+          Forall2 binding_inv_top xs vs2 /\
+          Forall2 (V i) vs1 vs2.
+    Proof.
+      intros HG xs.
+      intros.
+      induction xs; simpl; intros.
+      - eexists; eexists; repeat split; eauto.
+      - rewrite FromList_cons in H.
+        edestruct (G_top_get HG) as [v1 [v2 [Heqv1 [Heqv2 [Hb HV]]]]]; eauto.
+        eapply Disjoint_FromList_cons_inv in H0; inv H0; auto.
 
-  Lemma G_top_get_list {i Γ1 ρ1 Γ2 ρ2} :
-    G_top i Γ1 ρ1 Γ2 ρ2 ->
-    forall xs,
-      (FromList xs) \subset Γ1 ->
-      Disjoint _ (FromList xs) (Dom_map K) ->
-      exists vs1 vs2,
-        get_list xs ρ1 = Some vs1 /\
-        get_list xs ρ2 = Some vs2 /\
-        Forall exposed vs2 /\
-        Forall2 binding_inv_top xs vs2 /\
-        Forall2 (V i) vs1 vs2.
-  Proof.
-    intros HG xs.
-    intros.
-    induction xs; simpl; intros.
-    - eexists; eexists; repeat split; eauto.
-    - rewrite FromList_cons in H.
-      edestruct (G_top_get HG) as [v1 [v2 [Heqv1 [Heqv2 [Hb HV]]]]]; eauto.
-      eapply Disjoint_FromList_cons_inv in H0; inv H0; auto.
+        edestruct IHxs as [vs1 [vs2 [Heqvs1 [Heqvs2 [Hexs [Hbs HVs]]]]]]; eauto.
+        eapply Included_trans; eauto.
+        apply Included_Union_r.
 
-      edestruct IHxs as [vs1 [vs2 [Heqvs1 [Heqvs2 [Hexs [Hbs HVs]]]]]]; eauto.
-      eapply Included_trans; eauto.
-      apply Included_Union_r.
+        rewrite Heqv1.
+        rewrite Heqvs1.
+        rewrite Heqv2.
+        rewrite Heqvs2.
+        exists (v1 :: vs1), (v2 :: vs2); repeat (split; auto).
+        constructor; auto.
+        inv Hb.
+        inv H3; auto.
+    Qed.
 
-      rewrite Heqv1.
-      rewrite Heqvs1.
-      rewrite Heqv2.
-      rewrite Heqvs2.
-      exists (v1 :: vs1), (v2 :: vs2); repeat (split; auto).
-      constructor; auto.
-      inv Hb.
-      inv H3; auto.
-  Qed.
+    Lemma G_top_set {i Γ1 ρ1 Γ2 ρ2}:
+      G_top i Γ1 ρ1 Γ2 ρ2 ->
+      forall {x v1 v2},
+        binding_inv_top x v2 ->
+        V i v1 v2 ->
+        G_top i (x |: Γ1) (M.set x v1 ρ1) (x |: Γ2) (M.set x v2 ρ2).
+    Proof.
+      intros.
+      unfold G_top; intros.
 
-  Lemma G_top_set {i Γ1 ρ1 Γ2 ρ2}:
-    G_top i Γ1 ρ1 Γ2 ρ2 ->
-    forall {x v1 v2},
-      binding_inv_top x v2 ->
-      V i v1 v2 ->
-      G_top i (x |: Γ1) (M.set x v1 ρ1) (x |: Γ2) (M.set x v2 ρ2).
-  Proof.
-    intros.
-    unfold G_top; intros.
+      split.
+      eapply wf_env_set; eauto.
+      eapply G_top_wf_env_r; eauto.
+      eapply V_wf_val_r; eauto.
 
-    split.
-    eapply wf_env_set; eauto.
-    eapply G_top_wf_env_r; eauto.
-    eapply V_wf_val_r; eauto.
+      split.
+      apply Included_Union_compat; auto.
+      apply Included_refl.
+      eapply G_top_subset_inv; eauto.
 
-    split.
-    apply Included_Union_compat; auto.
-    apply Included_refl.
-    eapply G_top_subset_inv; eauto.
+      intros.
+      destruct (M.elt_eq x0 x); subst.
+      - repeat rewrite M.gss.
+        inv H0.
+        eexists; eexists; repeat split; eauto.
+      - repeat (rewrite M.gso; auto).
+        eapply G_top_get; eauto.
+        inv H2; auto.
+        inv H3; contradiction.
+    Qed.
 
-    intros.
-    destruct (M.elt_eq x0 x); subst.
-    - repeat rewrite M.gss.
-      inv H0.
+    Lemma G_top_set_lists {i Γ1 ρ1 Γ2 ρ2}:
+      G_top i Γ1 ρ1 Γ2 ρ2 ->
+      forall {xs vs1 vs2 ρ3 ρ4},
+        Forall2 (V i) vs1 vs2 ->
+        Forall2 binding_inv_top xs vs2 ->
+        set_lists xs vs1 ρ1 = Some ρ3 ->
+        set_lists xs vs2 ρ2 = Some ρ4 ->
+        G_top i (FromList xs :|: Γ1) ρ3 (FromList xs :|: Γ2) ρ4.
+    Proof.
+      intros HG xs.
+      assert (HΓ : Γ2 \subset Γ1) by (eapply G_top_subset_inv; eauto).
+      induction xs; simpl; intros.
+      - destruct vs1; try discriminate.
+        destruct vs2; try discriminate.
+        inv H1; inv H2.
+        eapply G_top_subset; eauto.
+        normalize_sets.
+        rewrite Union_Empty_set_neut_l; eauto.
+        apply Included_refl.
+        eapply Included_Union_compat; eauto.
+        apply Included_refl.
+      - destruct vs1; try discriminate.
+        destruct vs2; try discriminate.
+        destruct (set_lists xs vs1 ρ1) eqn:Heq1; try discriminate.
+        destruct (set_lists xs vs2 ρ2) eqn:Heq2; try discriminate.
+        inv H; inv H0; inv H1; inv H2.
+        eapply G_top_subset with (Γ1 := (a |: (FromList xs :|: Γ1))) (Γ2 := (a |: (FromList xs :|: Γ2))); eauto.
+        eapply G_top_set; eauto.
+        normalize_sets.
+        rewrite Union_assoc.
+        apply Included_refl.
+        eapply Included_Union_compat; eauto.
+        apply Included_refl.
+    Qed.
+
+    (* Monotonicity Lemma *)
+    Lemma G_top_mono {Γ1 Γ2 ρ1 ρ2} i j:
+      G_top i Γ1 ρ1 Γ2 ρ2 ->
+      j <= i ->
+      G_top j Γ1 ρ1 Γ2 ρ2.
+    Proof.
+      unfold G_top.
+      intros.
+      destruct H as [Hr2 [HS HG]].
+      repeat (split; auto); intros.
+      edestruct HG as [v1 [v2 [Heqv1 [Heqv2 [[Hk Hex] HV]]]]]; eauto.
       eexists; eexists; repeat split; eauto.
-    - repeat (rewrite M.gso; auto).
-      eapply G_top_get; eauto.
-      inv H2; auto.
-      inv H3; contradiction.
-  Qed.
+      apply V_mono with i; eauto.
+    Qed.
 
-  Lemma G_top_set_lists {i Γ1 ρ1 Γ2 ρ2}:
-    G_top i Γ1 ρ1 Γ2 ρ2 ->
-    forall {xs vs1 vs2 ρ3 ρ4},
-      Forall2 (V i) vs1 vs2 ->
-      Forall2 binding_inv_top xs vs2 ->
-      set_lists xs vs1 ρ1 = Some ρ3 ->
-      set_lists xs vs2 ρ2 = Some ρ4 ->
-      G_top i (FromList xs :|: Γ1) ρ3 (FromList xs :|: Γ2) ρ4.
-  Proof.
-    intros HG xs.
-    assert (HΓ : Γ2 \subset Γ1) by (eapply G_top_subset_inv; eauto).
-    induction xs; simpl; intros.
-    - destruct vs1; try discriminate.
-      destruct vs2; try discriminate.
-      inv H1; inv H2.
-      eapply G_top_subset; eauto.
-      normalize_sets.
-      rewrite Union_Empty_set_neut_l; eauto.
-      apply Included_refl.
-      eapply Included_Union_compat; eauto.
-      apply Included_refl.
-    - destruct vs1; try discriminate.
-      destruct vs2; try discriminate.
-      destruct (set_lists xs vs1 ρ1) eqn:Heq1; try discriminate.
-      destruct (set_lists xs vs2 ρ2) eqn:Heq2; try discriminate.
-      inv H; inv H0; inv H1; inv H2.
-      eapply G_top_subset with (Γ1 := (a |: (FromList xs :|: Γ1))) (Γ2 := (a |: (FromList xs :|: Γ2))); eauto.
+    (* Compatibility Lemmas *)
+    Lemma Vfun_V_top e e' :
+      known_map_inv K ->
+      trans_correct_top e e' ->
+      forall i f xs Γ1 Γ2 ρ1 ρ2,
+        K ! f = None ->
+        Disjoint _ (FromList xs) (Dom_map K) ->
+
+        G_top i Γ1 ρ1 Γ2 ρ2 ->
+        A0.occurs_free e \subset (FromList xs :|: (f |: Γ1)) ->
+        A1.occurs_free e' \subset (FromList xs :|: (f |: Γ2)) ->
+        V i (A0.Vfun f ρ1 xs e) (Tag w0 (A1.Vfun f ρ2 xs e')).
+    Proof.
+      unfold trans_correct_top.
+      intros HK [HS He] i.
+      assert (Hw0 : w0 \in Exposed) by (apply w0_exposed).
+
+      induction i; simpl; intros; auto;
+        assert (Hρ2 : wf_env ρ2) by (eapply G_top_wf_env_r; eauto);
+        repeat (split; auto); intros;
+        destruct (K ! f) eqn:HKf; try discriminate;
+        split; auto; intros.
+
+      apply (He (i - (i - j)) ρ3 ρ4); auto.
+      eapply G_top_subset with (Γ1 := FromList xs :|: (f |: Γ1)) (Γ2 := FromList xs :|: (f |: Γ2)); eauto.
+      eapply G_top_set_lists; eauto.
       eapply G_top_set; eauto.
-      normalize_sets.
-      rewrite Union_assoc.
-      apply Included_refl.
-      eapply Included_Union_compat; eauto.
-      apply Included_refl.
-  Qed.
+      eapply G_top_mono; eauto; try lia.
+      eapply binding_inv_top_exposed; simpl; eauto.
+      apply V_mono with i; try lia.
+      eapply IHi with (Γ2 := Γ2); eauto.
+      apply G_top_mono with (S i); eauto; lia.
+      eapply binding_inv_top_exposed_Forall; eauto.
+      eapply set_lists_length_eq; eauto.
+    Qed.
 
-  (* Monotonicity Lemma *)
-  Lemma G_top_mono {Γ1 Γ2 ρ1 ρ2} i j:
-    G_top i Γ1 ρ1 Γ2 ρ2 ->
-    j <= i ->
-    G_top j Γ1 ρ1 Γ2 ρ2.
-  Proof.
-    unfold G_top.
-    intros.
-    destruct H as [Hr2 [HS HG]].
-    repeat (split; auto); intros.
-    edestruct HG as [v1 [v2 [Heqv1 [Heqv2 [[Hk Hex] HV]]]]]; eauto.
-    eexists; eexists; repeat split; eauto.
-    apply V_mono with i; eauto.
-  Qed.
+    Lemma free_fun_compat e e' f k k' xs :
+      A1.occurs_free e' \subset A0.occurs_free e ->
+      A1.occurs_free k' \subset A0.occurs_free k ->
+      A1.occurs_free (A1.Efun f w0 xs e' k') \subset A0.occurs_free (A0.Efun f xs e k).
+    Proof.
+      unfold Ensembles.Included, Ensembles.In.
+      intros.
+      inv H1; auto.
+    Qed.
 
-  (* Compatibility Lemmas *)
-  Lemma Vfun_V_top e e' :
-    known_map_inv K ->
-    trans_correct_top e e' ->
-    forall i f xs Γ1 Γ2 ρ1 ρ2,
+    Lemma fun_compat_top e e' k k' f xs :
       K ! f = None ->
       Disjoint _ (FromList xs) (Dom_map K) ->
 
-      G_top i Γ1 ρ1 Γ2 ρ2 ->
-      A0.occurs_free e \subset (FromList xs :|: (f |: Γ1)) ->
-      A1.occurs_free e' \subset (FromList xs :|: (f |: Γ2)) ->
-      V i (A0.Vfun f ρ1 xs e) (Tag w0 (A1.Vfun f ρ2 xs e')).
-  Proof.
-    unfold trans_correct_top.
-    intros HK [HS He] i.
-    assert (Hw0 : w0 \in Exposed) by (apply w0_exposed).
+      trans_correct_top e e' ->
+      trans_correct_top k k' ->
+      trans_correct_top (A0.Efun f xs e k) (Efun f w0 xs e' k').
+    Proof.
+      unfold trans_correct_top, E, E'.
+      intros HKf HKxs; intros.
+      assert (Hw0 : w0 \in Exposed) by (apply w0_exposed).
 
-    induction i; simpl; intros; auto;
-      assert (Hρ2 : wf_env ρ2) by (eapply G_top_wf_env_r; eauto);
-      repeat (split; auto); intros;
-      destruct (K ! f) eqn:HKf; try discriminate;
-      split; auto; intros.
+      destruct H.
+      destruct H0.
+      split; intros.
+      eapply free_fun_compat; eauto.
 
-    apply (He (i - (i - j)) ρ3 ρ4); auto.
-    eapply G_top_subset with (Γ1 := FromList xs :|: (f |: Γ1)) (Γ2 := FromList xs :|: (f |: Γ2)); eauto.
-    eapply G_top_set_lists; eauto.
-    eapply G_top_set; eauto.
-    eapply G_top_mono; eauto; try lia.
-    eapply binding_inv_top_exposed; simpl; eauto.
-    apply V_mono with i; try lia.
-    eapply IHi with (Γ2 := Γ2); eauto.
-    apply G_top_mono with (S i); eauto; lia.
-    eapply binding_inv_top_exposed_Forall; eauto.
-    eapply set_lists_length_eq; eauto.
-  Qed.
+      inv H6.
+      - exists 0, OOT; split; simpl; eauto.
+      - inv H7.
+        edestruct (H2 (i - 1) (M.set f (A0.Vfun f ρ1 xs e) ρ1) (M.set f (Tag w0 (A1.Vfun f ρ2 xs e')) ρ2)) with (j1 := c) (r1 := r1) as [j2 [r2 [Hk2 Rr]]]; eauto; try lia.
+        + eapply G_top_subset with (Γ1 := (f |: (A0.occurs_free (A0.Efun f xs e k)))) (Γ2 := (f |: (A1.occurs_free (A1.Efun f w0 xs e' k')))); eauto.
+          * eapply G_top_set; eauto.
+            eapply G_top_mono; eauto; try lia.
+            split; auto.
 
-  Lemma free_fun_compat e e' f k k' xs :
-    A1.occurs_free e' \subset A0.occurs_free e ->
-    A1.occurs_free k' \subset A0.occurs_free k ->
-    A1.occurs_free (A1.Efun f w0 xs e' k') \subset A0.occurs_free (A0.Efun f xs e k).
-  Proof.
-    unfold Ensembles.Included, Ensembles.In.
-    intros.
-    inv H1; auto.
-  Qed.
+            eapply Vfun_V_top with (Γ1 := (A0.occurs_free (A0.Efun f xs e k))) (Γ2 := (A1.occurs_free (A1.Efun f w0 xs e' k'))); eauto.
+            -- unfold trans_correct_top.
+               split; auto.
+            -- eapply G_top_mono; eauto; try lia.
+            -- eapply A0.free_fun_e_subset; eauto.
+            -- eapply A1.free_fun_e_subset; eauto.
+          * eapply A0.free_fun_k_subset; eauto.
+        + exists (S j2), r2; split; auto.
+          * constructor; auto.
+            eapply bstep_fuel_exposed_inv; eauto.
+          * apply R_mono with ((i - 1) - c); try lia; auto.
+    Qed.
 
-  Lemma fun_compat_top e e' k k' f xs :
-    K ! f = None ->
-    Disjoint _ (FromList xs) (Dom_map K) ->
+    Lemma free_letapp_compat k k' f x xs :
+      A1.occurs_free k' \subset A0.occurs_free k ->
+      A1.occurs_free (A1.Eletapp x f w0 xs k') \subset A0.occurs_free (A0.Eletapp x f xs k).
+    Proof.
+      unfold Ensembles.Included, Ensembles.In.
+      intros.
+      inv H0; auto.
+    Qed.
 
-    trans_correct_top e e' ->
-    trans_correct_top k k' ->
-    trans_correct_top (A0.Efun f xs e k) (Efun f w0 xs e' k').
-  Proof.
-    unfold trans_correct_top, E, E'.
-    intros HKf HKxs; intros.
-    assert (Hw0 : w0 \in Exposed) by (apply w0_exposed).
+    Lemma letapp_compat_top k k' xs x f :
+      K ! f = None ->
+      Disjoint _ (FromList xs) (Dom_map K) ->
+      K ! x = None ->
 
-    destruct H.
-    destruct H0.
-    split; intros.
-    eapply free_fun_compat; eauto.
+      trans_correct_top k k' ->
+      trans_correct_top (A0.Eletapp x f xs k) (A1.Eletapp x f w0 xs k').
+    Proof.
+      unfold trans_correct_top, E, E'.
+      intros HKf HKxs HKx; intros.
+      destruct H.
+      split; intros.
+      eapply free_letapp_compat; eauto.
 
-    inv H6.
-    - exists 0, OOT; split; simpl; eauto.
-    - inv H7.
-      edestruct (H2 (i - 1) (M.set f (A0.Vfun f ρ1 xs e) ρ1) (M.set f (Tag w0 (A1.Vfun f ρ2 xs e')) ρ2)) with (j1 := c) (r1 := r1) as [j2 [r2 [Hk2 Rr]]]; eauto; try lia.
-      + eapply G_top_subset with (Γ1 := (f |: (A0.occurs_free (A0.Efun f xs e k)))) (Γ2 := (f |: (A1.occurs_free (A1.Efun f w0 xs e' k')))); eauto.
-        * eapply G_top_set; eauto.
-          eapply G_top_mono; eauto; try lia.
-          split; auto.
+      inv H4.
+      - exists 0, OOT; split; simpl; auto.
+      - inv H5.
+        + edestruct (G_top_get H2) as [fv1 [fv2 [Heqfv1 [Heqfv2 [[_ Hexfv] HVf]]]]]; eauto.
+          rewrite Heqfv1 in H9; inv H9.
+          destruct fv2.
+          destruct i.
+          inv H3.
+          simpl in HVf.
+          destruct HVf as [Hfv2 HV]; subst.
+          destruct v0; try contradiction.
+          destruct HV as [Heqf [Hlen HV]]; subst.
+          rename v0 into f'.
+          inv Hexfv.
+          destruct (K ! f') eqn:HKf'.
+          destruct HV as [Heqw [Hexw' _]]; subst; contradiction.
 
-          eapply Vfun_V_top with (Γ1 := (A0.occurs_free (A0.Efun f xs e k))) (Γ2 := (A1.occurs_free (A1.Efun f w0 xs e' k'))); eauto.
-          -- unfold trans_correct_top.
-             split; auto.
-          -- eapply G_top_mono; eauto; try lia.
-          -- eapply A0.free_fun_e_subset; eauto.
-          -- eapply A1.free_fun_e_subset; eauto.
-        * eapply A0.free_fun_k_subset; eauto.
-      + exists (S j2), r2; split; auto.
-        * constructor; auto.
-          eapply bstep_fuel_exposed_inv; eauto.
-        * apply R_mono with ((i - 1) - c); try lia; auto.
-  Qed.
+          destruct HV as [Hex HV].
 
-  Lemma free_letapp_compat k k' f x xs :
-    A1.occurs_free k' \subset A0.occurs_free k ->
-    A1.occurs_free (A1.Eletapp x f w0 xs k') \subset A0.occurs_free (A0.Eletapp x f xs k).
-  Proof.
-    unfold Ensembles.Included, Ensembles.In.
-    intros.
-    inv H0; auto.
-  Qed.
+          edestruct (G_top_get_list H2 xs) as [vs1 [vs2 [Heqvs1 [Heqvs2 [Hexs [Hbs HVvs]]]]]]; eauto.
+          eapply A0.free_letapp_xs_subset; eauto.
 
-  Lemma letapp_compat_top k k' xs x f :
-    K ! f = None ->
-    Disjoint _ (FromList xs) (Dom_map K) ->
-    K ! x = None ->
+          rewrite Heqvs1 in H10; inv H10.
 
-    trans_correct_top k k' ->
-    trans_correct_top (A0.Eletapp x f xs k) (A1.Eletapp x f w0 xs k').
-  Proof.
-    unfold trans_correct_top, E, E'.
-    intros HKf HKxs HKx; intros.
-    destruct H.
-    split; intros.
-    eapply free_letapp_compat; eauto.
+          assert (Heqw : w = w0) by (eapply Exposed_singleton; eauto); inv Heqw.
 
-    inv H4.
-    - exists 0, OOT; split; simpl; auto.
-    - inv H5.
-      + edestruct (G_top_get H2) as [fv1 [fv2 [Heqfv1 [Heqfv2 [[_ Hexfv] HVf]]]]]; eauto.
-        rewrite Heqfv1 in H9; inv H9.
-        destruct fv2.
-        destruct i.
-        inv H3.
-        simpl in HVf.
-        destruct HVf as [Hfv2 HV]; subst.
-        destruct v0; try contradiction.
-        destruct HV as [Heqf [Hlen HV]]; subst.
-        rename v0 into f'.
-        inv Hexfv.
-        destruct (K ! f') eqn:HKf'.
-        destruct HV as [Heqw [Hexw' _]]; subst; contradiction.
+          destruct (set_lists_length3 (M.set f' (Tag w0 (Vfun f' t l e0)) t) l vs2) as [ρ4 Heqρ4].
+          unfold wval in *.
+          rewrite <- (Forall2_length _ _ _ HVvs).
+          rewrite <- (set_lists_length_eq _ _ _ _ H13); auto.
 
-        destruct HV as [Hex HV].
+          unfold E' in HV.
+          edestruct (HV i vs vs2 ρ'' ρ4) with (j1 := c0) as [j2 [r2 [He0 HR]]]; eauto; try lia.
+          * eapply V_mono_Forall; eauto; lia.
+          * destruct r2; simpl in HR; try contradiction.
+            edestruct (H0 (i - c0) (M.set x v ρ1) (M.set x w ρ2)) with (j1 := c') as [j3 [r3 [He1 HR']]]; eauto; try lia.
+            eapply G_top_subset with (Γ1 := x |: (A0.occurs_free (A0.Eletapp x f xs k))) (Γ2 := x |: (A1.occurs_free (A1.Eletapp x f w0 xs k'))); eauto.
+            eapply G_top_set; eauto.
+            eapply G_top_mono; eauto; lia.
+            -- eapply binding_inv_top_exposed; eauto.
+               assert (Hw : exposed_res (A1.Res w)) by (eapply bstep_fuel_exposed_inv; eauto); inv Hw; auto.
+            -- eapply V_mono; eauto; try lia.
+            -- eapply A0.free_letapp_k_subset; eauto.
+            -- exists (S (j2 + j3)), r3; split; eauto.
+               2 : { eapply R_mono; eauto; lia. }
 
-        edestruct (G_top_get_list H2 xs) as [vs1 [vs2 [Heqvs1 [Heqvs2 [Hexs [Hbs HVvs]]]]]]; eauto.
-        eapply A0.free_letapp_xs_subset; eauto.
+               constructor; auto.
+               eapply BStep_letapp_Res with (v := w); eauto.
+               destruct (exposed_reflect w0); try contradiction; auto.
 
-        rewrite Heqvs1 in H10; inv H10.
+               intros.
+               split; auto.
+               assert (Hw : exposed_res (A1.Res w)) by (eapply bstep_fuel_exposed_inv; eauto); inv Hw; auto.
 
-        assert (Heqw : w = w0) by (eapply Exposed_singleton; eauto); inv Heqw.
+               eapply bstep_fuel_exposed_inv; eauto.
+        + eexists; exists OOT; split; simpl; eauto.
+    Qed.
 
-        destruct (set_lists_length3 (M.set f' (Tag w0 (Vfun f' t l e0)) t) l vs2) as [ρ4 Heqρ4].
-        unfold wval in *.
-        rewrite <- (Forall2_length _ _ _ HVvs).
-        rewrite <- (set_lists_length_eq _ _ _ _ H13); auto.
+    (* Linking Preservation *)
+    Definition linking_inv f x :=
+      K ! f = None /\ K ! x = None.
 
-        unfold E' in HV.
-        edestruct (HV i vs vs2 ρ'' ρ4) with (j1 := c0) as [j2 [r2 [He0 HR]]]; eauto; try lia.
-        * eapply V_mono_Forall; eauto; lia.
-        * destruct r2; simpl in HR; try contradiction.
-          edestruct (H0 (i - c0) (M.set x v ρ1) (M.set x w ρ2)) with (j1 := c') as [j3 [r3 [He1 HR']]]; eauto; try lia.
-          eapply G_top_subset with (Γ1 := x |: (A0.occurs_free (A0.Eletapp x f xs k))) (Γ2 := x |: (A1.occurs_free (A1.Eletapp x f w0 xs k'))); eauto.
-          eapply G_top_set; eauto.
-          eapply G_top_mono; eauto; lia.
-          -- eapply binding_inv_top_exposed; eauto.
-             assert (Hw : exposed_res (A1.Res w)) by (eapply bstep_fuel_exposed_inv; eauto); inv Hw; auto.
-          -- eapply V_mono; eauto; try lia.
-          -- eapply A0.free_letapp_k_subset; eauto.
-          -- exists (S (j2 + j3)), r3; split; eauto.
-             2 : { eapply R_mono; eauto; lia. }
-
-             constructor; auto.
-             eapply BStep_letapp_Res with (v := w); eauto.
-             destruct (exposed_reflect w0); try contradiction; auto.
-
-             intros.
-             split; auto.
-             assert (Hw : exposed_res (A1.Res w)) by (eapply bstep_fuel_exposed_inv; eauto); inv Hw; auto.
-
-             eapply bstep_fuel_exposed_inv; eauto.
-      + eexists; exists OOT; split; simpl; eauto.
-  Qed.
-
-  (* Linking Preservation *)
-  (* To link two programs, we take a joined `K` that knows about both programs.
+    (* To link two programs, we take a joined `K` that knows about both programs.
      Note this is general enough to cover the ideal scenario when `e1` and `e1'` have distinct bound identifiers *)
-  Lemma preserves_linking f w x e1 e2 e1' e2' :
-    K ! f = None ->
-    K ! x = None ->
-    (w \in Exposed) ->
-    trans_correct_top e1 e2 ->
-    trans_correct_top e1' e2' ->
-    trans_correct_top (A0.link f x e1 e1') (A1.link f w x e2 e2').
-  Proof.
-    unfold A0.link, A1.link.
-    intros.
-    apply Exposed_singleton in H1; subst.
-    eapply fun_compat_top; eauto.
-    normalize_sets.
-    eapply Disjoint_Empty_set_l; eauto.
-    eapply letapp_compat_top; eauto.
-    normalize_sets.
-    eapply Disjoint_Empty_set_l; eauto.
-  Qed.
+    Lemma preserves_linking f w x e1 e2 e1' e2' :
+      linking_inv f x ->
+      (w \in Exposed) ->
+      trans_correct_top e1 e2 ->
+      trans_correct_top e1' e2' ->
+      trans_correct_top (A0.link f x e1 e1') (A1.link f w x e2 e2').
+    Proof.
+      unfold A0.link, A1.link.
+      intros [HKf HKx]; intros.
+      apply Exposed_singleton in H; subst.
+      eapply fun_compat_top; eauto.
+      normalize_sets.
+      eapply Disjoint_Empty_set_l; eauto.
+      eapply letapp_compat_top; eauto.
+      normalize_sets.
+      eapply Disjoint_Empty_set_l; eauto.
+    Qed.
 
-End Known.
+  End Known.
+
+End M.
