src/Framework/Annotate.v
@@ -6,100 +6,116 @@ Module A1 := ANF.
 
 Module Type Annotate.
 
+  (* Analysis result type *)
+  Parameter web_map : Type.
+
+  (* Analysis result invariant used by transformation *)
+  Parameter web_map_inv : web_map -> Prop.
+
+  (* Analysis result specification *)
+  Parameter analysis_spec : web_map -> A0.exp -> Prop.
+
   (* For any Annotate pass, it should produce at least one exposed web ids *)
   Parameter Exposed_nonempty : exists w, w \in Exposed.
 
   (* Specification *)
-  Parameter trans : A0.vars -> A0.exp -> A1.exp -> Prop.
+  Parameter trans : web_map -> A0.vars -> A0.exp -> A1.exp -> Prop.
 
-  (* For any Annotate pass, if e is an invalid program,
-     we can always annotate the entire program with the trivial annotation to make trans complete. *)
+  (* A successful analysis should always allow us to transform the program *)
   Parameter trans_total :
-    forall e1,
+    forall W e1,
+      web_map_inv W ->
+      analysis_spec W e1 ->
       exists e2,
-        Annotate.trans (A0.occurs_free e1) e1 e2.
+        trans W (A0.occurs_free e1) e1 e2.
 
-  (* Erase o Annotate = id *)
-  Parameter Erase_Annotate_id :
-    forall e1 e2 e1',
-      Annotate.trans (A0.occurs_free e1) e1 e1' ->
+  (* `Erase` is left inverse of `trans` *)
+  (* `Erase o Annotate = id` *)
+  Parameter trans_erase :
+    forall W e1 e2 e1',
+      Annotate.trans W (A0.occurs_free e1) e1 e1' ->
       Erase.trans (A1.occurs_free e1') e1' e2 ->
       e1 = e2.
 
   (* Cross-language Logical Relations *)
-  Parameter V : nat -> A0.val -> A1.wval -> Prop.
+  Parameter V : web_map -> nat -> A0.val -> A1.wval -> Prop.
 
   Parameter V_wf_val_r :
-    forall i v1 v2,
-      V i v1 v2 ->
+    forall W i v1 v2,
+      V W i v1 v2 ->
       wf_val v2.
 
-  Parameter R : nat -> A0.res -> A1.res -> Prop.
+  Parameter R : web_map -> nat -> A0.res -> A1.res -> Prop.
 
   Parameter R_res_inv_l :
-    forall i v1 r2,
-      R i (A0.Res v1) r2 ->
-      exists v2, r2 = A1.Res v2 /\ V i v1 v2.
+    forall W i v1 r2,
+      R W i (A0.Res v1) r2 ->
+      exists v2, r2 = A1.Res v2 /\ V W i v1 v2.
 
   (* Top-level Logical Relations *)
-  Parameter G_top : nat -> A0.vars -> A0.env -> A1.vars -> A1.env -> Prop.
+  Parameter G_top : web_map -> nat -> A0.vars -> A0.env -> A1.vars -> A1.env -> Prop.
 
   Parameter G_top_wf_env_r :
-    forall i Γ1 ρ1 Γ2 ρ2,
-      G_top i Γ1 ρ1 Γ2 ρ2 ->
+    forall W i Γ1 ρ1 Γ2 ρ2,
+      G_top W i Γ1 ρ1 Γ2 ρ2 ->
       wf_env ρ2.
 
   Parameter G_top_subset :
-    forall i Γ1 ρ1 Γ2 ρ2 Γ3 Γ4,
-      G_top i Γ1 ρ1 Γ2 ρ2 ->
+    forall W i Γ1 ρ1 Γ2 ρ2 Γ3 Γ4,
+      G_top W i Γ1 ρ1 Γ2 ρ2 ->
       Γ3 \subset Γ1 ->
       Γ4 \subset Γ3 ->
-      G_top i Γ3 ρ1 Γ4 ρ2.
+      G_top W i Γ3 ρ1 Γ4 ρ2.
 
-  Parameter trans_correct_top : A0.exp -> A1.exp -> Prop.
+  Parameter trans_correct_top : web_map -> A0.exp -> A1.exp -> Prop.
 
   Parameter top :
-    forall e1 e2,
-      trans (A0.occurs_free e1) e1 e2 ->
-      trans_correct_top e1 e2.
+    forall W e1 e2,
+      trans W (A0.occurs_free e1) e1 e2 ->
+      trans_correct_top W e1 e2.
 
   Parameter trans_correct_top_subset :
-    forall e1 e2,
-      trans_correct_top e1 e2 ->
+    forall W e1 e2,
+      trans_correct_top W e1 e2 ->
       A1.occurs_free e2 \subset A0.occurs_free e1.
 
   (* Adequacy *)
   Parameter adequacy :
-    forall e1 e2,
-      trans_correct_top e1 e2 ->
+    forall W e1 e2,
+      web_map_inv W ->
+      trans_correct_top W e1 e2 ->
       forall ρ1 ρ2,
         wf_env ρ2 ->
-        (forall k, G_top k (A0.occurs_free e1) ρ1 (A1.occurs_free e2) ρ2) ->
+        (forall k, G_top W k (A0.occurs_free e1) ρ1 (A1.occurs_free e2) ρ2) ->
         forall j1 r1,
           A0.bstep_fuel ρ1 e1 j1 r1 ->
           exists j2 r2,
             A1.bstep_fuel true ρ2 e2 j2 r2 /\
-            (forall k, R k r1 r2).
+            (forall k, R W k r1 r2).
 
   (* Behavioral Refinement *)
   Parameter val_ref : A0.val -> A1.wval -> Prop.
 
   Parameter V_val_ref :
-    forall v1 v2,
-      (forall i, V i v1 v2) ->
+    forall W v1 v2,
+      (forall i, V W i v1 v2) ->
       val_ref v1 v2.
 
   Parameter R_res_val_ref :
-    forall v1 v2,
-      (forall i, R i (A0.Res v1) (A1.Res v2)) ->
+    forall W v1 v2,
+      (forall i, R W i (A0.Res v1) (A1.Res v2)) ->
       val_ref v1 v2.
+
+  (* Preconditions for linking *)
+  Parameter linking_inv : web_map -> var -> var -> Prop.
 
   (* Linking Preservation *)
   Parameter preserves_linking :
-    forall f w x e1 e2 e1' e2',
+    forall W f w x e1 e2 e1' e2',
+      linking_inv W f x ->
       (w \in Exposed) ->
-      trans_correct_top e1 e2 ->
-      trans_correct_top e1' e2' ->
-      trans_correct_top (A0.link f x e1 e1') (A1.link f w x e2 e2').
+      trans_correct_top W e1 e2 ->
+      trans_correct_top W e1' e2' ->
+      trans_correct_top W (A0.link f x e1 e1') (A1.link f w x e2 e2').
 
 End Annotate.
